WIP

src/example/TicketLockW.v
@@ -343,6 +343,25 @@ Section SIM.
   Variable tk_mono: nat.
   Variable wm_mono: nat.
 
+  (* Definition ticket_lock_inv_unlocking *)
+  (*            (l: list thread_id) (tks: NatMap.t nat) (now next: nat) (myt: thread_id) : iProp := *)
+  (*   (own_thread myt) *)
+  (*     ∗ *)
+  (*     (⌜tkqueue l tks (S now) next⌝) *)
+  (*     ∗ *)
+  (*     (natmap_prop_sum tks (fun th tk => FairRA.white th (Ord.from_nat (tk - (S now))))) *)
+  (*     ∗ *)
+  (*     (list_prop_sum (fun th => ((ObligationRA.duty (inl th) []) *)
+  (*                               ∗ (∃ u, maps_to th (Auth.black (Excl.just u: Excl.t nat))))%I) l) *)
+  (*     ∗ *)
+  (*     (∃ (k: nat) (o: Ord.t), *)
+  (*         (monoBlack monok mypreord (now, Tkst.d k)) *)
+  (*           ∗ (ObligationRA.black k o) *)
+  (*           ∗ (ObligationRA.pending k 1) *)
+  (*           ∗ (ObligationRA.duty (inl myt) [(k, Ord.S Ord.O)]) *)
+  (*     ) *)
+  (* . *)
+
   Definition ticket_lock_inv_unlocking
              (l: list thread_id) (tks: NatMap.t nat) (now next: nat) (myt: thread_id) : iProp :=
     (own_thread myt)
@@ -354,11 +373,8 @@ Section SIM.
       (list_prop_sum (fun th => ((ObligationRA.duty (inl th) [])
                                 ∗ (∃ u, maps_to th (Auth.black (Excl.just u: Excl.t nat))))%I) l)
       ∗
-      (∃ (k: nat) (o: Ord.t),
-          (monoBlack monok mypreord (now, Tkst.d k))
-            ∗ (ObligationRA.black k o)
-            ∗ (ObligationRA.pending k 1)
-            ∗ (ObligationRA.duty (inl myt) [(k, Ord.S Ord.O)])
+      (∃ (k: nat),
+          (monoBlack monok mypreord (now, Tkst.c k))
       )
   .
 
@@ -442,52 +458,53 @@ Section SIM.
   .
 
   Definition ticket_lock_inv_state
-             (mem: WMem.t) (own: bool) (V: TView.t) (tks: NatMap.t nat) : iProp :=
-    ((St_tgt (tt, mem)) ∗ (St_src ((own, V), (key_set tks))))
+             (mem: WMem.t) (own: bool) (svw: TView.t) (ing: bool) (tks: NatMap.t nat) : iProp :=
+    ((St_tgt (tt, mem)) ∗ (St_src (((own, svw), ing), (key_set tks))))
   .
 
   Definition ticket_lock_inv : iProp :=
-    ∃ (mem: WMem.t) (own: bool) (V: TView.t) (wk: nat)
+    ∃ (mem: WMem.t) (own ing: bool) (V svw: TView.t) (wk: nat)
       (l: list thread_id) (tks: NatMap.t nat) (now next: nat) (myt: thread_id),
       (ticket_lock_inv_tks tks)
         ∗
-        (ticket_lock_inv_mem mem V wk now next myt)
+        ((ticket_lock_inv_mem mem V wk now next myt) ∗ (⌜TView.le V svw⌝))
         ∗
-        ((ticket_lock_inv_state mem own V tks))
+        ((ticket_lock_inv_state mem own svw ing tks))
         ∗
         (((⌜own = true⌝)
-            ∗ (ticket_lock_inv_locked l tks now next myt V)
+            ∗ (((⌜ing = false⌝) ∗ (ticket_lock_inv_locked l tks now next myt V))
+               ∨
+                 ((⌜ing = true⌝) ∗ (ticket_lock_inv_unlocking l tks now next myt))
+              )
          )
          ∨
            ((⌜own = false⌝)
-              ∗ ((ticket_lock_inv_unlocking l tks now next myt)
-                 ∨
-                   ((ticket_lock_inv_unlocked0 l tks now next myt V)
-                    ∨
-                      (ticket_lock_inv_unlocked1 l tks now next myt V))
-                )
+              ∗
+              (⌜ing = false⌝)
+              ∗ 
+              ((ticket_lock_inv_unlocked0 l tks now next myt V)
+               ∨
+                 (ticket_lock_inv_unlocked1 l tks now next myt V))
         ))
   .
 
   Let I: list iProp := [ticket_lock_inv].
 
-  (* TODO *)
-
   (* Properties *)
-  Lemma unlocking_mono
-        l tks now next myt:
-    (ticket_lock_inv_unlocking l tks now next myt)
-      -∗
-      ((⌜tkqueue l tks (S now) next⌝)
-         ∗
-         (∃ k o, (monoWhite monok mypreord (now, Tkst.d k))
-                   ∗ (ObligationRA.black k o)
-      )).
-  Proof.
-    iIntros "I". iDestruct "I" as "[_ [%I2 [_ [_ I]]]]". do 2 iDestruct "I" as "[% I]".
-    iDestruct "I" as "[MB [OB _]]". iPoseProof (black_white with "MB") as "#MYTURN".
-    iSplit. auto. iExists k, o. iFrame. auto.
-  Qed.
+  (* Lemma unlocking_mono *)
+  (*       l tks now next myt: *)
+  (*   (ticket_lock_inv_unlocking l tks now next myt) *)
+  (*     -∗ *)
+  (*     ((⌜tkqueue l tks (S now) next⌝) *)
+  (*        ∗ *)
+  (*        (∃ k o, (monoWhite monok mypreord (now, Tkst.d k)) *)
+  (*                  ∗ (ObligationRA.black k o) *)
+  (*     )). *)
+  (* Proof. *)
+  (*   iIntros "I". iDestruct "I" as "[_ [%I2 [_ [_ I]]]]". do 2 iDestruct "I" as "[% I]". *)
+  (*   iDestruct "I" as "[MB [OB _]]". iPoseProof (black_white with "MB") as "#MYTURN". *)
+  (*   iSplit. auto. iExists k, o. iFrame. auto. *)
+  (* Qed. *)
 
   Lemma unlocking_contra
         tid l tks now next myt
@@ -511,24 +528,24 @@ Section SIM.
       -∗ ⌜False⌝.
   Proof.
     iIntros "MYT I". iDestruct "I" as "[_ [%I2 [_ [_ I3]]]]".
-    do 2 (iDestruct "I3" as "[% I3]"). iDestruct "I3" as "[I3 _]".
+    do 1 (iDestruct "I3" as "[% I3]").
     iPoseProof (black_white_compare with "MYT I3") as "%LE". exfalso.
     hexploit (tkqueue_val_range_l I2 _ FIND). i. inv LE; try lia.
   Qed.
 
   Lemma unlocked0_contra
-        tid l tks now next myt mytk
+        tid l tks now next myt mytk V
         (FIND: NatMap.find tid tks = Some mytk)
     :
-    (ticket_lock_inv_unlocked0 l tks now next myt)
+    (ticket_lock_inv_unlocked0 l tks now next myt V)
       -∗ ⌜False⌝.
   Proof.
     iIntros "I". iDestruct "I" as "[_ [%I2 _]]". exfalso. des; clarify.
   Qed.
 
   Lemma unlocked1_mono
-        l tks now next myt:
-    (ticket_lock_inv_unlocked1 l tks now next myt)
+        l tks now next myt V:
+    (ticket_lock_inv_unlocked1 l tks now next myt V)
       -∗
       ((⌜tkqueue l tks now next⌝)
          ∗
@@ -542,13 +559,13 @@ Section SIM.
   Qed.
 
   Lemma unlocked1_myturn
-        tid l tks now next myt
+        tid l tks now next myt V
         mytk o
         (FIND: NatMap.find tid tks = Some mytk)
     :
     (monoWhite monok mypreord (mytk, o))
       -∗
-      (ticket_lock_inv_unlocked1 l tks now next myt)
+      (ticket_lock_inv_unlocked1 l tks now next myt V)
       -∗ ⌜now = mytk⌝.
   Proof.
     iIntros "MYT I". do 2 iDestruct "I" as "[% I]". iDestruct "I" as "[_ [%I1 [%I2 [_ [_ I]]]]]".
@@ -558,10 +575,10 @@ Section SIM.
   Qed.
 
   Lemma locked_contra
-        tid l tks now next myt
+        tid l tks now next myt V
         (FIND: NatMap.find tid tks = Some now)
     :
-    (ticket_lock_inv_locked l tks now next myt)
+    (ticket_lock_inv_locked l tks now next myt V)
       -∗ ⌜False⌝.
   Proof.
     iIntros "I". iDestruct "I" as "[_ [%I2 _]]". exfalso.
@@ -569,13 +586,13 @@ Section SIM.
   Qed.
 
   Lemma locked_myturn
-        tid l tks now next myt
+        tid l tks now next myt V
         mytk o
         (FIND: NatMap.find tid tks = Some mytk)
     :
     (monoWhite monok mypreord (mytk, o))
       -∗
-      (ticket_lock_inv_locked l tks now next myt)
+      (ticket_lock_inv_locked l tks now next myt V)
       -∗ ⌜False⌝.
   Proof.
     iIntros "MYT I". iDestruct "I" as "[_ [%I2 [_ [_ [% I3]]]]]".
@@ -593,78 +610,105 @@ Section SIM.
   Qed.
 
   Lemma ticket_lock_inv_mem_mono
-        mem now next myt
+        mem now next myt V wk
     :
-    (ticket_lock_inv_mem mem now next myt)
+    (ticket_lock_inv_mem mem V wk now next myt)
       -∗
       (monoWhite tk_mono Nat.le_preorder now).
   Proof.
-    iIntros "MEM". iDestruct "MEM" as "[MEM0 [MEM1 [MEM2 [MEM3 MEM4]]]]".
+    iIntros "MEM". iDestruct "MEM" as "[MEM0 [MEM1 [MEM2 [MEM3 [MEM4 MEM5]]]]]".
     iPoseProof (black_white with "MEM4") as "#MONOTK".
     auto.
   Qed.
 
+  Lemma ticket_lock_inv_mem_mono2
+        mem now next myt V wk
+    :
+    (ticket_lock_inv_mem mem V wk now next myt)
+      -∗
+      (monoWhite wm_mono wmpreord (now, wk)).
+  Proof.
+    iIntros "MEM". iDestruct "MEM" as "[MEM0 [MEM1 [MEM2 [MEM3 [MEM4 [MEM5 MEM6]]]]]]".
+    iPoseProof (black_white with "MEM5") as "#MONOTK".
+    auto.
+  Qed.
+
   (* Simulations *)
-  Lemma lock_enqueue tid:
+  Lemma lock_enqueue tid tvw:
     ((own_thread tid)
        ∗ (ObligationRA.duty (inl tid) [])
     )
       ∗
-      (∀ mytk,
+      (∀ mytk tview,
           (
             (OwnM (Auth.white (NatMapRA.singleton tid mytk: NatMapRA.t TicketLockW.tk)))
               ∗ (maps_to tid (Auth.white (Excl.just 2: Excl.t nat)))
           )
-          -∗
+            -∗
   (stsim I tid (topset I) ibot7 ibot7
-         (λ r_src r_tgt : (), (own_thread tid ** ObligationRA.duty (inl tid) []) ** ⌜r_src = r_tgt⌝)
+         (λ r_src r_tgt : TView.t, (own_thread tid ** ObligationRA.duty (inl tid) []) ** ⌜r_src = r_tgt⌝)
          false false
     (ITree.iter
-        (λ _ : (),
-           trigger Yield;;;
-           ` x_0 : bool * NatMap.t () <- trigger (Get (bool * NatMap.t ()));;
-           (let (own0, _) := x_0 in if Bool.eqb own0 true then Ret (inl ()) else Ret (inr ())))
-        ();;;
-      ` x_0 : bool * NatMap.t () <- trigger (Get (bool * NatMap.t ()));;
-      (let (_, ts0) := x_0 in
-       trigger (Put (true, NatMap.remove (elt:=()) tid ts0));;;
-       trigger
-         (Fair
-            (λ i : nat,
-               if tid_dec i tid
-               then Flag.success
-               else
-                if NatMapP.F.In_dec (NatMap.remove (elt:=()) tid ts0) i
-                then Flag.fail
-                else Flag.emp));;; trigger Yield;;; Ret ()))
-    (OMod.close_itree TicketLock.omod (WMem.mod TicketLock.gvs)
-       (TicketLock.lock_loop (WMem.val_nat mytk));;;
-     OMod.close_itree TicketLock.omod (WMem.mod TicketLock.gvs) (trigger Yield))
+       (λ _ : (),
+          trigger Yield;;;
+          ` x_ : bool * TView.t * bool * NatMap.t () <- trigger (Get (bool * TView.t * bool * NatMap.t ()));;
+          (let (y, _) := x_ in let (y1, _) := y in let (own, _) := y1 in if own then Ret (inl ()) else Ret (inr ()))) ();;;
+     ` x_ : bool * TView.t * bool * NatMap.t () <- trigger (Get (bool * TView.t * bool * NatMap.t ()));;
+     (let (y, ts) := x_ in
+      let (y0, ing) := y in
+      let (_, tvw_lock) := y0 in
+      if ing
+      then ` x : _ <- trigger (Choose void);; Empty_set_rect (λ _ : void, itree ((eventE +' cE) +' sE AbsLockW.st) TView.t) x
+      else
+       ` x_0 : {tvw' : TView.t | TView.le (TView.join tvw tvw_lock) tvw'} <-
+       trigger (Choose {tvw' : TView.t | TView.le (TView.join tvw tvw_lock) tvw'});;
+       (let (tvw', _) := x_0 in
+        trigger (Put (true, tvw', false, NatMap.remove (elt:=()) tid ts));;;
+        trigger
+          (Fair
+             (λ i : nat,
+                if tid_dec i tid
+                then Flag.success
+                else if NatMapP.F.In_dec (NatMap.remove (elt:=()) tid ts) i then Flag.fail else Flag.emp));;;
+        trigger Yield;;; Ret tvw')))
+    (` a : TView.t <- OMod.close_itree TicketLockW.omod WMem.mod (TicketLockW.lock_loop (nat2c mytk) tview);;
+     OMod.close_itree TicketLockW.omod WMem.mod (trigger Yield;;; Ret a))
   )
       )
       ⊢
       (stsim I tid (topset I) ibot7 ibot7
              (fun r_src r_tgt => own_thread tid ** ObligationRA.duty (inl tid) [] ** ⌜r_src = r_tgt⌝)
              false false
-             (AbsLock.lock_fun tt)
-             (OMod.close_itree TicketLock.omod (WMem.mod TicketLock.gvs)
-                               (TicketLock.lock_fun tt))).
+             (AbsLockW.lock_fun tvw)
+             (OMod.close_itree TicketLockW.omod (WMem.mod)
+                               (TicketLockW.lock_fun tvw))).
   Proof.
     iIntros "[[MYTH DUTY] SIM]".
-    unfold AbsLock.lock_fun, TicketLock.lock_fun. rred.
+    unfold AbsLockW.lock_fun, TicketLockW.lock_fun. rred.
     rewrite close_itree_call. rred.
     iApply (stsim_sync with "[DUTY]"). msubtac. iFrame. iIntros "DUTY _".
     unfold Mod.wrap_fun, WMem.faa_fun. rred.
     iApply stsim_tidL. lred.
 
-    iopen 0 "I" "K". do 7 iDestruct "I" as "[% I]". iDestruct "I" as "[TKS [MEM [ST CASES]]]".
+    iopen 0 "I" "K". do 11 iDestruct "I" as "[% I]". iDestruct "I" as "[TKS [MEM [ST CASES]]]".
     iDestruct "ST" as "[ST0 ST1]".
     iApply stsim_getL. iSplit. auto. iApply (stsim_putL with "ST1"). iIntros "ST1".
 
     iApply stsim_getR. iSplit. auto. rred. iApply stsim_tauR. rred.
-    iDestruct "MEM" as "[MEM0 [MEM1 [MEM2 MEM3]]]".
-    iPoseProof (memory_ra_faa with "MEM0 MEM2") as "[% [%FAA >[MEM0 MEM2]]]".
-    erewrite FAA. rred.
+    iDestruct "MEM" as "[MEM %VWLE]". iDestruct "MEM" as "[MEM0 [MEM1 [MEM2 MEM3]]]".
+    iApply stsim_chooseR. iIntros "%".
+    destruct x. destruct x as [[[[lc2 to] val] sc1] mem1]. des. rename y into READ, y0 into WRITE. rred.
+
+    iPoseProof (wmemory_ra_faa with "MEM0 MEM2") as "[%FAA >[MEM0 MEM2]]".
+    eapply READ. eapply WRITE. auto. auto.
+    iApply stsim_tauR. rred.
+    iApply stsim_fairR.
+    { i. instantiate (1:= []). ss. clear - IN. unfold sum_fmap_r, sum_fmap_l, WMem.missed in IN. des_ifs. }
+    { i. instantiate (1:=[]) in IN. inv IN. }
+    { econs. }
+    { auto. }
+    iIntros "_ _". rred.
+    iApply stsim_tauR. rred.
     iApply stsim_getR. iSplit. auto. rred.
     iApply (stsim_putR with "ST0"). iIntros "ST0". rred.
     iApply stsim_tauR. rred. iApply stsim_tauR. rred.
@@ -678,7 +722,7 @@ Section SIM.
     iDestruct "TKS" as "[TKS0 [TKS1 [TKS2 TKS3]]]".
     set (tks' := NatMap.add tid next tks).
     iPoseProof (NatMapRA_add with "TKS0") as ">[TKS0 MYTK]". eauto. instantiate (1:=next).
-    iAssert (St_src (own, (key_set tks')))%I with "[ST1]" as "ST1".
+    iAssert (St_src (own, svw, ing, (key_set tks')))%I with "[ST1]" as "ST1".
     { subst tks'. rewrite key_set_pull_add_eq. iFrame. }
     iPoseProof ((FairRA.whites_unfold (fun id => ~ NatMap.In id tks') _ (i:=tid)) with "TKS1") as "[TKS1 MYTRI]".
     { subst tks'. i. ss. des; clarify.
@@ -707,59 +751,60 @@ Section SIM.
     iAssert (natmap_prop_sum tks' (λ tid0 _ : nat, own_thread tid0))%I with "[MYTH TKS2]" as "TKS2".
     { subst tks'. iApply (natmap_prop_sum_add with "TKS2"). iFrame. }
 
-    iDestruct "CASES" as "[[%TRUE INV] | [%FALSE INV]]"; subst.
+    iDestruct "CASES" as "[[%TRUE [[%IF INV] | [%IT INV]]] | [%FALSE [%IF [INV | INV]]]]"; subst.
     { iPoseProof (FairRA.white_mon with "MYTRI") as ">MYTRI".
-      { instantiate (1:=Ord.from_nat (next - (S now))). ss.
-        apply Ord.lt_le. apply Ord.omega_upperbound.
-      }
+      { instantiate (1:=Ord.from_nat (next - (S now))). ss. apply Ord.lt_le. apply Ord.omega_upperbound. }
       iMod ("K" with "[DUTY TKS0 TKS1 TKS2 TKS3 MEM0 MEM1 MEM2 MEM3 INV ST0 ST1 MYTRI MYNB]") as "_".
       { subst tks'. unfold ticket_lock_inv.
-        iExists m1, true, (l ++ [tid]), (NatMap.add tid next tks), now, (S next), myt.
+        iExists _, true, false, V, svw, wk, (l ++ [tid]), (NatMap.add tid next tks). iExists now, (S next), myt.
         iFrame.
         iSplitL "MEM2".
-        { ss. replace (S next) with (next + 1). iFrame. lia. }
-        iLeft. iSplit; auto. unfold ticket_lock_inv_locked.
+        { iSplit. 2: auto. replace (nat2c (S next)) with (Const.add (nat2c next) const_1). iFrame.
+          unfold nat2c. ss. clear. unfold BinIntDef.Z.of_nat. des_ifs. ss. rewrite Z.add_comm. rewrite Pos2Z.add_pos_pos.
+          rewrite Pplus_one_succ_l. econs.
+        }
+        iLeft. iSplit. auto. iLeft. iSplit. auto. unfold ticket_lock_inv_locked.
         iDestruct "INV" as "[INV0 [INV1 [INV2 [INV3 INV4]]]]". iFrame.
         iSplit.
         { iPure "INV1" as ?. iPureIntro. apply tkqueue_enqueue; auto. }
         iPoseProof (natmap_prop_sum_add with "INV2 MYTRI") as "INV2". iFrame.
         iApply list_prop_sum_add. iFrame. iExists 2. iFrame.
       }
-      iApply stsim_reset. iApply "SIM". iFrame.
+      iApply stsim_reset. destruct lc2. ss. des. subst val. iApply "SIM". iFrame.
     }
 
-    iDestruct "INV" as "[INV | INV]".
     { iPoseProof (FairRA.white_mon with "MYTRI") as ">MYTRI".
-      { instantiate (1:=Ord.from_nat (next - (S now))). ss.
-        apply Ord.lt_le. apply Ord.omega_upperbound.
-      }
+      { instantiate (1:=Ord.from_nat (next - (S now))). ss. apply Ord.lt_le. apply Ord.omega_upperbound. }
       iMod ("K" with "[DUTY TKS0 TKS1 TKS2 TKS3 MEM0 MEM1 MEM2 MEM3 INV ST0 ST1 MYTRI MYNB]") as "_".
       { subst tks'. unfold ticket_lock_inv.
-        iExists m1, false, (l ++ [tid]), (NatMap.add tid next tks), now, (S next), myt.
-    remember ((⌜false = true⌝ **
-     ticket_lock_inv_locked (l ++ [tid]) (NatMap.add tid next tks) now (S next) myt)
-    ∨ (⌜false = false⌝ **
-       ticket_lock_inv_unlocking (l ++ [tid]) (NatMap.add tid next tks) now (S next) myt
-       ∨ ticket_lock_inv_unlocked0 (l ++ [tid]) (NatMap.add tid next tks) now (S next) myt
-         ∨ ticket_lock_inv_unlocked1 (l ++ [tid]) (NatMap.add tid next tks) now (S next) myt))%I as temp.
+        iExists _, true, true, V, svw, wk, (l ++ [tid]), (NatMap.add tid next tks). iExists now, (S next), myt.
+        remember (
+    (⌜true = true⌝ **
+     (⌜true = false⌝ ** ticket_lock_inv_locked (l ++ [tid]) (NatMap.add tid next tks) now (S next) myt V)
+     ∨ (⌜true = true⌝ ** ticket_lock_inv_unlocking (l ++ [tid]) (NatMap.add tid next tks) now (S next) myt))
+    ∨ (⌜true = false⌝ **
+       (⌜true = false⌝ **
+        ticket_lock_inv_unlocked0 (l ++ [tid]) (NatMap.add tid next tks) now (S next) myt V
+        ∨ ticket_lock_inv_unlocked1 (l ++ [tid]) (NatMap.add tid next tks) now (S next) myt V))
+          )%I as temp.
         iFrame. subst temp.
         iSplitL "MEM2".
-        { ss. replace (S next) with (next + 1). iFrame. lia. }
-        iRight. iSplit; auto. iLeft. unfold ticket_lock_inv_unlocking.
+        { iSplit. 2: auto. replace (nat2c (S next)) with (Const.add (nat2c next) const_1). iFrame.
+          unfold nat2c. ss. clear. unfold BinIntDef.Z.of_nat. des_ifs. ss. rewrite Z.add_comm. rewrite Pos2Z.add_pos_pos.
+          rewrite Pplus_one_succ_l. econs.
+        }
+        iLeft. iSplit. auto. iRight. iSplit. auto. unfold ticket_lock_inv_unlocking.
         iDestruct "INV" as "[INV0 [INV1 [INV2 [INV3 INV4]]]]". iFrame.
         iSplit.
         { iPure "INV1" as ?. iPureIntro. apply tkqueue_enqueue; auto. }
         iPoseProof (natmap_prop_sum_add with "INV2 MYTRI") as "INV2". iFrame.
         iApply list_prop_sum_add. iFrame. iExists 2. iFrame.
       }
-      iApply stsim_reset. iApply "SIM". iFrame.
+      iApply stsim_reset. destruct lc2. ss. des. subst val. iApply "SIM". iFrame.
     }
 
-    iDestruct "INV" as "[INV | INV]".
     { iPoseProof (FairRA.white_mon with "MYTRI") as ">MYTRI".
-      { instantiate (1:=Ord.from_nat (next - (now))). ss.
-        apply Ord.lt_le. apply Ord.omega_upperbound.
-      }
+      { instantiate (1:=Ord.from_nat (next - (now))). ss. apply Ord.lt_le. apply Ord.omega_upperbound. }
       iPoseProof (ObligationRA.alloc (((Ord.S Ord.O) × Ord.omega) × (Ord.from_nat 3))%ord) as "> [% [[OBLK OWHI] OPEND]]".
       iPoseProof (ObligationRA.white_eq with "OWHI") as "OWHI".
       { rewrite Ord.from_nat_S. rewrite Jacobsthal.mult_S. reflexivity. }
@@ -771,18 +816,23 @@ Section SIM.
 
       iMod ("K" with "[DUTY TKS0 TKS1 TKS2 TKS3 MEM0 MEM1 MEM2 MEM3 INV0 INV2 ST0 ST1 MYTRI MYNB OBLK OPEND TAX]") as "_".
       { subst tks'. unfold ticket_lock_inv.
-        iExists m1, false, (l ++ [tid]), (NatMap.add tid next tks), now, (S next), myt.
-    remember ((⌜false = true⌝ **
-     ticket_lock_inv_locked (l ++ [tid]) (NatMap.add tid next tks) now (S next) myt)
-    ∨ (⌜false = false⌝ **
-       ticket_lock_inv_unlocking (l ++ [tid]) (NatMap.add tid next tks) now (S next) myt
-       ∨ ticket_lock_inv_unlocked0 (l ++ [tid]) (NatMap.add tid next tks) now (S next) myt
-         ∨ ticket_lock_inv_unlocked1 (l ++ [tid]) (NatMap.add tid next tks) now (S next) myt))%I as temp.
+        iExists _, false, false, V, svw, wk, (l ++ [tid]), (NatMap.add tid next tks). iExists now, (S next), myt.
+        remember (
+    (⌜true = true⌝ **
+     (⌜true = false⌝ ** ticket_lock_inv_locked (l ++ [tid]) (NatMap.add tid next tks) now (S next) myt V)
+     ∨ (⌜true = true⌝ ** ticket_lock_inv_unlocking (l ++ [tid]) (NatMap.add tid next tks) now (S next) myt))
+    ∨ (⌜true = false⌝ **
+       (⌜true = false⌝ **
+        ticket_lock_inv_unlocked0 (l ++ [tid]) (NatMap.add tid next tks) now (S next) myt V
+        ∨ ticket_lock_inv_unlocked1 (l ++ [tid]) (NatMap.add tid next tks) now (S next) myt V))
+          )%I as temp.
         iFrame. subst temp.
         iSplitL "MEM2".
-        { ss. replace (S next) with (next + 1). iFrame. lia. }
-        iRight. iSplit; auto. iRight. iRight.
-        unfold ticket_lock_inv_unlocked1.
+        { iSplit. 2: auto. replace (nat2c (S next)) with (Const.add (nat2c next) const_1). iFrame.
+          unfold nat2c. ss. clear. unfold BinIntDef.Z.of_nat. des_ifs. ss. rewrite Z.add_comm. rewrite Pos2Z.add_pos_pos.
+          rewrite Pplus_one_succ_l. econs.
+        }
+        iRight. iSplit. auto. iSplit. auto. iRight. unfold ticket_lock_inv_unlocked1.
         des; clarify. ss. iExists tid, []. ss. iFrame.
         iSplit; auto.
         iSplit.
@@ -791,26 +841,30 @@ Section SIM.
         }
         iSplitR. auto. iExists k, _, 2. iFrame.
       }
-      iApply stsim_reset. iApply "SIM". iFrame.
+      iApply stsim_reset. destruct lc2. ss. des. subst val. iApply "SIM". iFrame.
     }
 
     { iPoseProof (FairRA.white_mon with "MYTRI") as ">MYTRI".
-      { instantiate (1:=Ord.from_nat (next - (now))). ss.
-        apply Ord.lt_le. apply Ord.omega_upperbound.
-      }
+      { instantiate (1:=Ord.from_nat (next - (now))). ss. apply Ord.lt_le. apply Ord.omega_upperbound. }
       iMod ("K" with "[DUTY TKS0 TKS1 TKS2 TKS3 MEM0 MEM1 MEM2 MEM3 INV ST0 ST1 MYTRI MYNB]") as "_".
       { subst tks'. unfold ticket_lock_inv.
-        iExists m1, false, (l ++ [tid]), (NatMap.add tid next tks), now, (S next), myt.
-    remember ((⌜false = true⌝ **
-     ticket_lock_inv_locked (l ++ [tid]) (NatMap.add tid next tks) now (S next) myt)
-    ∨ (⌜false = false⌝ **
-       ticket_lock_inv_unlocking (l ++ [tid]) (NatMap.add tid next tks) now (S next) myt
-       ∨ ticket_lock_inv_unlocked0 (l ++ [tid]) (NatMap.add tid next tks) now (S next) myt
-         ∨ ticket_lock_inv_unlocked1 (l ++ [tid]) (NatMap.add tid next tks) now (S next) myt))%I as temp.
+        iExists _, false, false, V, svw, wk, (l ++ [tid]), (NatMap.add tid next tks). iExists now, (S next), myt.
+        remember (
+    (⌜true = true⌝ **
+     (⌜true = false⌝ ** ticket_lock_inv_locked (l ++ [tid]) (NatMap.add tid next tks) now (S next) myt V)
+     ∨ (⌜true = true⌝ ** ticket_lock_inv_unlocking (l ++ [tid]) (NatMap.add tid next tks) now (S next) myt))
+    ∨ (⌜true = false⌝ **
+       (⌜true = false⌝ **
+        ticket_lock_inv_unlocked0 (l ++ [tid]) (NatMap.add tid next tks) now (S next) myt V
+        ∨ ticket_lock_inv_unlocked1 (l ++ [tid]) (NatMap.add tid next tks) now (S next) myt V))
+          )%I as temp.
         iFrame. subst temp.
         iSplitL "MEM2".
-        { ss. replace (S next) with (next + 1). iFrame. lia. }
-        iRight. iSplit; auto. iRight. iRight. unfold ticket_lock_inv_unlocked1.
+        { iSplit. 2: auto. replace (nat2c (S next)) with (Const.add (nat2c next) const_1). iFrame.
+          unfold nat2c. ss. clear. unfold BinIntDef.Z.of_nat. des_ifs. ss. rewrite Z.add_comm. rewrite Pos2Z.add_pos_pos.
+          rewrite Pplus_one_succ_l. econs.
+        }
+        iRight. iSplit; auto. iSplit. auto. iRight. unfold ticket_lock_inv_unlocked1.
         do 2 iDestruct "INV" as "[% INV]".
         iDestruct "INV" as "[INV0 [% [INV2 [INV3 [INV4 INV5]]]]]". subst.
         iExists yourt, (waits ++ [tid]). ss. iFrame.
@@ -820,7 +874,7 @@ Section SIM.
         iPoseProof (natmap_prop_sum_add with "INV3 MYTRI") as "INV3". iFrame.
         iApply list_prop_sum_add. iFrame. iExists 2. iFrame.
       }
-      iApply stsim_reset. iApply "SIM". iFrame.
+      iApply stsim_reset. destruct lc2. ss. des. subst val. iApply "SIM". iFrame.
     }
   Qed.
 
@@ -832,11 +886,11 @@ Section SIM.
             → itree ((eventE +' cE) +' sE (Mod.state AbsLockW.mod)) R_src
             → itree
                 ((eventE +' cE) +'
-                                   sE (OMod.closed_state TicketLock.omod (WMem.mod TicketLock.gvs))) R_tgt
+                                   sE (OMod.closed_state TicketLockW.omod (WMem.mod))) R_tgt
             → iProp)
         (ps pt: bool)
         (src: itree ((eventE +' cE) +' sE (Mod.state AbsLockW.mod)) unit)
-        (tgt: itree ((eventE +' cE) +' sE (OMod.closed_state TicketLock.omod (WMem.mod TicketLock.gvs))) unit)
+        (tgt: itree ((eventE +' cE) +' sE (OMod.closed_state TicketLockW.omod (WMem.mod))) unit)
         (tid mytk u: nat)
         x
     :
@@ -865,9 +919,9 @@ Section SIM.
     (trigger Yield;;; tgt)).
   Proof.
     iIntros "[[MYTK [MYNW MYTURN]] SIM]".
-    iopen 0 "I" "K". do 7 iDestruct "I" as "[% I]". iDestruct "I" as "[TKS [MEM [ST CASES]]]".
+    iopen 0 "I" "K". do 11 iDestruct "I" as "[% I]". iDestruct "I" as "[TKS [MEM [ST CASES]]]".
     iPoseProof (mytk_find_some with "[MYTK TKS]") as "%FIND". iFrame.
-    iDestruct "CASES" as "[[%CT I] | [%CF [I | [I | I]]]]".
+    iDestruct "CASES" as "[[%CT [[% I] | [% I]]] | [%CF [%CF2 [I | I]]]]".
     { iPoseProof (locked_myturn with "MYTURN I") as "%FF". eauto. inv FF. }
     { iPoseProof (unlocking_myturn with "MYTURN I") as "%FF". eauto. inv FF. }
     { iPoseProof (unlocked0_contra with "I") as "%FF". eauto. inv FF. }
@@ -899,15 +953,17 @@ Section SIM.
     { iFrame. iApply ObligationRA.tax_cons_fold. iFrame. }
     iIntros "I8 _".
     iMod ("K" with "[TKS MEM ST I0 I3 I4 I5 I6 I7 I8 I9 I10]") as "_".
-    { iExists mem, false, (tid :: tl), tks, now, next, myt.
+    { unfold ticket_lock_inv. iExists mem, false, false, V, svw, wk, (tid :: tl), tks. iExists now, next, myt.
       remember (
-          (⌜false = true⌝ ** ticket_lock_inv_locked (tid :: tl) tks now next myt)
-          ∨ (⌜false = false⌝ **
-                           ticket_lock_inv_unlocking (tid :: tl) tks now next myt
-             ∨ ticket_lock_inv_unlocked0 (tid :: tl) tks now next myt
-             ∨ ticket_lock_inv_unlocked1 (tid :: tl) tks now next myt))%I as temp.
+    (⌜false = true⌝ **
+     (⌜false = false⌝ ** ticket_lock_inv_locked (tid :: tl) tks now next myt V)
+     ∨ (⌜false = true⌝ ** ticket_lock_inv_unlocking (tid :: tl) tks now next myt))
+    ∨ (⌜false = false⌝ **
+       (⌜false = false⌝ **
+        ticket_lock_inv_unlocked0 (tid :: tl) tks now next myt V ∨ ticket_lock_inv_unlocked1 (tid :: tl) tks now next myt V))
+        )%I as temp.
       iFrame. subst temp.
-      iRight. iSplit. auto. iRight. iRight.
+      iRight. iSplit. auto. iSplit. auto. iRight.
       iExists tid, tl. iFrame. iSplit. auto. iSplit. auto.
       iExists k, o, u. iFrame.
     }
@@ -922,27 +978,28 @@ Section SIM.
             → itree ((eventE +' cE) +' sE (Mod.state AbsLockW.mod)) R_src
             → itree
                 ((eventE +' cE) +'
-                                   sE (OMod.closed_state TicketLock.omod (WMem.mod TicketLock.gvs))) R_tgt
+                                   sE (OMod.closed_state TicketLockW.omod (WMem.mod))) R_tgt
             → iProp)
         (ps pt: bool)
         (src: itree ((eventE +' cE) +' sE (Mod.state AbsLockW.mod)) unit)
-        (tgt: itree ((eventE +' cE) +' sE (OMod.closed_state TicketLock.omod (WMem.mod TicketLock.gvs))) unit)
+        (tgt: itree ((eventE +' cE) +' sE (OMod.closed_state TicketLockW.omod (WMem.mod))) unit)
         (tid mytk now: nat)
-        tks mem next l myt own
+        tks mem next l myt own V wk svw ing
+        (VW: TView.le V svw)
         (NEQ: mytk <> now)
     :
   (OwnM (Auth.white (NatMapRA.singleton tid mytk: NatMapRA.t nat)) **
     (ticket_lock_inv_tks tks **
-     (ticket_lock_inv_mem mem now next myt **
-      (ticket_lock_inv_state mem own tks **
-       ((⌜own = true⌝ ** ticket_lock_inv_locked l tks now next myt)
-        ∨ (⌜own = false⌝ **
-           ticket_lock_inv_unlocking l tks now next myt
-           ∨ ticket_lock_inv_unlocked0 l tks now next myt
-             ∨ ticket_lock_inv_unlocked1 l tks now next myt) **
+     (ticket_lock_inv_mem mem V wk now next myt **
+      (ticket_lock_inv_state mem own svw ing tks **
+       ((⌜own = true⌝ **
+           (⌜ing = false⌝ ** ticket_lock_inv_locked l tks now next myt V)
+           ∨ (⌜ing = true⌝ ** ticket_lock_inv_unlocking l tks now next myt))
+          ∨ (⌜own = false⌝ **
+             (⌜ing = false⌝ ** ticket_lock_inv_unlocked0 l tks now next myt V ∨ ticket_lock_inv_unlocked1 l tks now next myt V)) **
         (ticket_lock_inv -*
          MUpd (nth_default True%I I)
-           (fairI (ident_tgt:=OMod.closed_ident TicketLock.omod (WMem.mod TicketLock.gvs))) []
+           (fairI (ident_tgt:=OMod.closed_ident TicketLockW.omod (WMem.mod))) []
            [0] True))))))
       ∗
       (((OwnM (Auth.white ((NatMapRA.singleton tid mytk: NatMapRA.t nat))))
@@ -963,37 +1020,38 @@ Section SIM.
   Proof.
     iIntros "[[MYTH [TKS [MEM [ST [CASES K]]]]] SIM]".
     iPoseProof (mytk_find_some with "[MYTH TKS]") as "%FIND". iFrame.
-    iDestruct "CASES" as "[[CT INV]|[CF INV]]".
+    iDestruct "CASES" as "[[CT [[IF INV] | [IT INV]]]|[CF [IF [INV | INV]]]]".
     { unfold ticket_lock_inv_locked. iDestruct "INV" as "[INV0 [%INV1 [INV2 [INV3 INV4]]]]".
       hexploit (tkqueue_find_in INV1 _ FIND). i.
       iPoseProof (list_prop_sum_in_split with "INV3") as "[[DUTY MAPS] INV3]". eapply H.
       iApply (stsim_yieldR_strong with "[DUTY]"). iFrame. iIntros "DUTY RIGHT".
-      iMod ("K" with "[TKS MEM ST CT INV0 INV2 INV4 MAPS INV3 DUTY]") as "_".
-      { iExists mem, own, l, tks, now, next, myt.
-        remember 
-    ((⌜own = true⌝ ** ticket_lock_inv_locked l tks now next myt)
+      iMod ("K" with "[TKS MEM ST CT IF INV0 INV2 INV4 MAPS INV3 DUTY]") as "_".
+      { unfold ticket_lock_inv. iExists mem, own, ing, V, svw, wk, l, tks. iExists now, next, myt.
+        remember (
+    (⌜own = true⌝ **
+     (⌜ing = false⌝ ** ticket_lock_inv_locked l tks now next myt V) ∨ (⌜ing = true⌝ ** ticket_lock_inv_unlocking l tks now next myt))
     ∨ (⌜own = false⌝ **
-       ticket_lock_inv_unlocking l tks now next myt
-       ∨ ticket_lock_inv_unlocked0 l tks now next myt
-       ∨ ticket_lock_inv_unlocked1 l tks now next myt))%I as temp. iFrame. subst temp.
-        iLeft. iSplit. auto. iFrame. iSplit. auto. iApply "INV3". iFrame.
+                   (⌜ing = false⌝ ** ticket_lock_inv_unlocked0 l tks now next myt V ∨ ticket_lock_inv_unlocked1 l tks now next myt V))
+          )%I as temp.
+        iFrame. iSplit. auto. subst temp.
+        iLeft. iSplit. auto. iFrame. iLeft. iSplit. auto. iFrame. iSplit. auto. iApply "INV3". iFrame.
       }
       iModIntro. iApply "SIM". iFrame.
     }
-    iDestruct "INV" as "[INV | [INV | INV]]".
     { iDestruct "INV" as "[INV0 [%INV1 [INV2 [INV3 INV4]]]]".
       hexploit (tkqueue_find_in INV1 _ FIND). i.
       iPoseProof (list_prop_sum_in_split with "INV3") as "[[DUTY MAPS] INV3]". eapply H.
       iApply (stsim_yieldR_strong with "[DUTY]"). iFrame. iIntros "DUTY RIGHT".
-      iMod ("K" with "[TKS MEM ST CF INV0 INV2 INV4 MAPS INV3 DUTY]") as "_".
-      { iExists mem, own, l, tks, now, next, myt.
-        remember 
-    ((⌜own = true⌝ ** ticket_lock_inv_locked l tks now next myt)
+      iMod ("K" with "[TKS MEM ST CT IT INV0 INV2 INV4 MAPS INV3 DUTY]") as "_".
+      { iExists mem, own, ing, V, svw, wk, l, tks. iExists now, next, myt.
+        remember (
+    (⌜own = true⌝ **
+     (⌜ing = false⌝ ** ticket_lock_inv_locked l tks now next myt V) ∨ (⌜ing = true⌝ ** ticket_lock_inv_unlocking l tks now next myt))
     ∨ (⌜own = false⌝ **
-       ticket_lock_inv_unlocking l tks now next myt
-       ∨ ticket_lock_inv_unlocked0 l tks now next myt
-       ∨ ticket_lock_inv_unlocked1 l tks now next myt))%I as temp. iFrame. subst temp.
-        iRight. iSplit. auto. iLeft. iFrame. iSplit. auto. iApply "INV3". iFrame.
+                   (⌜ing = false⌝ ** ticket_lock_inv_unlocked0 l tks now next myt V ∨ ticket_lock_inv_unlocked1 l tks now next myt V))
+          )%I as temp.
+        iFrame. iSplit. auto. subst temp.
+        iLeft. iSplit. auto. iFrame. iRight. iSplit. auto. iFrame. iSplit. auto. iApply "INV3". iFrame.
       }
       iModIntro. iApply "SIM". iFrame.
     }
@@ -1008,529 +1066,530 @@ Section SIM.
       intro IN.
       iPoseProof (list_prop_sum_in_split with "INV4") as "[[DUTY MAPS] INV4]". eapply IN.
       iApply (stsim_yieldR_strong with "[DUTY]"). iFrame. iIntros "DUTY RIGHT".
-      iMod ("K" with "[TKS MEM ST CF INV0 INV3 INV5 MAPS INV4 DUTY]") as "_".
-      { iExists mem, own, l, tks, now, next, myt.
-        remember 
-    ((⌜own = true⌝ ** ticket_lock_inv_locked l tks now next myt)
+      iMod ("K" with "[TKS MEM ST CF IF INV0 INV3 INV5 MAPS INV4 DUTY]") as "_".
+      { iExists mem, own, ing, V, svw, wk, l, tks. iExists now, next, myt.
+        remember (
+    (⌜own = true⌝ **
+     (⌜ing = false⌝ ** ticket_lock_inv_locked l tks now next myt V) ∨ (⌜ing = true⌝ ** ticket_lock_inv_unlocking l tks now next myt))
     ∨ (⌜own = false⌝ **
-       ticket_lock_inv_unlocking l tks now next myt
-       ∨ ticket_lock_inv_unlocked0 l tks now next myt
-       ∨ ticket_lock_inv_unlocked1 l tks now next myt))%I as temp. iFrame. subst temp.
-        iRight. iSplit. auto. iRight. iRight. iFrame. iExists yourt, waits.
+                   (⌜ing = false⌝ ** ticket_lock_inv_unlocked0 l tks now next myt V ∨ ticket_lock_inv_unlocked1 l tks now next myt V))
+          )%I as temp.
+        iFrame. iSplit. auto. subst temp.
+        iRight. iSplit. auto. iSplit. auto. iRight. iFrame. iExists yourt, waits.
         iSplit. auto. iSplit. auto. iFrame. iApply "INV4". iFrame.
       }
       iModIntro. iApply "SIM". iFrame.
     }
   Qed.
 
-  Lemma lock_myturn0
-        (g0 g1 : ∀ R_src R_tgt : Type,
-            (R_src → R_tgt → iProp)
-            → bool
-            → bool
-            → itree ((eventE +' cE) +' sE (Mod.state AbsLockW.mod)) R_src
-            → itree ((eventE +' cE) +' sE (OMod.closed_state TicketLock.omod (WMem.mod TicketLock.gvs))) R_tgt → iProp)
-        (ps pt: bool)
-        (tid : nat)
-        (mytk : TicketLockW.tk)
-        x tx
-        (TX: 1 <= tx)
-    :
-    ((monoWhite monok mypreord (mytk, x))
-       ∗ (OwnM (Auth.white (NatMapRA.singleton tid mytk: NatMapRA.t nat)))
-       ∗ (maps_to tid (Auth.white (Excl.just tx: Excl.t nat))))
-  ⊢ stsim I tid (topset I) g0 g1
-      (λ r_src r_tgt : (), (own_thread tid ** ObligationRA.duty (inl tid) []) ** ⌜r_src = r_tgt⌝)
-      ps pt
-      (trigger Yield;;;
-       ` x : () + () <-
-       (` x_0 : bool * NatMap.t () <- trigger (Get (bool * NatMap.t ()));;
-        (let (own0, _) := x_0 in if Bool.eqb own0 true then Ret (inl ()) else Ret (inr ())));;
-       match x with
-       | inl l0 =>
-           tau;; ITree.iter
-                   (λ _ : (),
-                      trigger Yield;;;
-                      ` x_0 : bool * NatMap.t () <- trigger (Get (bool * NatMap.t ()));;
-                      (let (own0, _) := x_0 in
-                       if Bool.eqb own0 true then Ret (inl ()) else Ret (inr ()))) l0
-       | inr r0 => Ret r0
-       end;;;
-       ` x_0 : bool * NatMap.t () <- trigger (Get (bool * NatMap.t ()));;
-       (let (_, ts0) := x_0 in
-        trigger (Put (true, NatMap.remove (elt:=()) tid ts0));;;
-        trigger
-          (Fair
-             (λ i : nat,
-                if tid_dec i tid
-                then Flag.success
-                else
-                 if NatMapP.F.In_dec (NatMap.remove (elt:=()) tid ts0) i
-                 then Flag.fail
-                 else Flag.emp));;; trigger Yield;;; Ret ()))
-      (` r : Any.t <-
-       OMod.embed_itree TicketLock.omod (WMem.mod TicketLock.gvs)
-         (Mod.wrap_fun WMem.load_fun (Any.upcast TicketLock.now_serving));;
-       ` x : WMem.val <- (tau;; unwrap (Any.downcast r));;
-       OMod.close_itree TicketLock.omod (WMem.mod TicketLock.gvs)
-         (` b : bool <- OMod.call "compare" (x, WMem.val_nat mytk);;
-          (if b then Ret () else tau;; TicketLock.lock_loop (WMem.val_nat mytk)));;;
-         OMod.close_itree TicketLock.omod (WMem.mod TicketLock.gvs) (trigger Yield)).
-  Proof.
-    iIntros "[#MYTN [MYTK MYNU]]". 
-    iopen 0 "I" "K". do 7 iDestruct "I" as "[% I]". iDestruct "I" as "[TKS [MEM [ST CASES]]]".
-    iPoseProof (mytk_find_some with "[MYTK TKS]") as "%FIND". iFrame.
-    iDestruct "CASES" as "[[%CT I] | [%CF [I | [I | I]]]]".
-    { iPoseProof (locked_myturn with "MYTN I") as "%FF". eauto. inv FF. }
-    { iPoseProof (unlocking_myturn with "MYTN I") as "%FF". eauto. inv FF. }
-    { iPoseProof (unlocked0_contra with "I") as "%FF". eauto. inv FF. }
-    iPoseProof (unlocked1_myturn with "MYTN I") as "%EQ". eauto. subst now.
+  (* Lemma lock_myturn0 *)
+  (*       (g0 g1 : ∀ R_src R_tgt : Type, *)
+  (*           (R_src → R_tgt → iProp) *)
+  (*           → bool *)
+  (*           → bool *)
+  (*           → itree ((eventE +' cE) +' sE (Mod.state AbsLockW.mod)) R_src *)
+  (*           → itree ((eventE +' cE) +' sE (OMod.closed_state TicketLock.omod (WMem.mod TicketLock.gvs))) R_tgt → iProp) *)
+  (*       (ps pt: bool) *)
+  (*       (tid : nat) *)
+  (*       (mytk : TicketLockW.tk) *)
+  (*       x tx *)
+  (*       (TX: 1 <= tx) *)
+  (*   : *)
+  (*   ((monoWhite monok mypreord (mytk, x)) *)
+  (*      ∗ (OwnM (Auth.white (NatMapRA.singleton tid mytk: NatMapRA.t nat))) *)
+  (*      ∗ (maps_to tid (Auth.white (Excl.just tx: Excl.t nat)))) *)
+  (* ⊢ stsim I tid (topset I) g0 g1 *)
+  (*     (λ r_src r_tgt : (), (own_thread tid ** ObligationRA.duty (inl tid) []) ** ⌜r_src = r_tgt⌝) *)
+  (*     ps pt *)
+  (*     (trigger Yield;;; *)
+  (*      ` x : () + () <- *)
+  (*      (` x_0 : bool * NatMap.t () <- trigger (Get (bool * NatMap.t ()));; *)
+  (*       (let (own0, _) := x_0 in if Bool.eqb own0 true then Ret (inl ()) else Ret (inr ())));; *)
+  (*      match x with *)
+  (*      | inl l0 => *)
+  (*          tau;; ITree.iter *)
+  (*                  (λ _ : (), *)
+  (*                     trigger Yield;;; *)
+  (*                     ` x_0 : bool * NatMap.t () <- trigger (Get (bool * NatMap.t ()));; *)
+  (*                     (let (own0, _) := x_0 in *)
+  (*                      if Bool.eqb own0 true then Ret (inl ()) else Ret (inr ()))) l0 *)
+  (*      | inr r0 => Ret r0 *)
+  (*      end;;; *)
+  (*      ` x_0 : bool * NatMap.t () <- trigger (Get (bool * NatMap.t ()));; *)
+  (*      (let (_, ts0) := x_0 in *)
+  (*       trigger (Put (true, NatMap.remove (elt:=()) tid ts0));;; *)
+  (*       trigger *)
+  (*         (Fair *)
+  (*            (λ i : nat, *)
+  (*               if tid_dec i tid *)
+  (*               then Flag.success *)
+  (*               else *)
+  (*                if NatMapP.F.In_dec (NatMap.remove (elt:=()) tid ts0) i *)
+  (*                then Flag.fail *)
+  (*                else Flag.emp));;; trigger Yield;;; Ret ())) *)
+  (*     (` r : Any.t <- *)
+  (*      OMod.embed_itree TicketLock.omod (WMem.mod TicketLock.gvs) *)
+  (*        (Mod.wrap_fun WMem.load_fun (Any.upcast TicketLock.now_serving));; *)
+  (*      ` x : WMem.val <- (tau;; unwrap (Any.downcast r));; *)
+  (*      OMod.close_itree TicketLock.omod (WMem.mod TicketLock.gvs) *)
+  (*        (` b : bool <- OMod.call "compare" (x, WMem.val_nat mytk);; *)
+  (*         (if b then Ret () else tau;; TicketLock.lock_loop (WMem.val_nat mytk)));;; *)
+  (*        OMod.close_itree TicketLock.omod (WMem.mod TicketLock.gvs) (trigger Yield)). *)
+  (* Proof. *)
+  (*   iIntros "[#MYTN [MYTK MYNU]]".  *)
+  (*   iopen 0 "I" "K". do 7 iDestruct "I" as "[% I]". iDestruct "I" as "[TKS [MEM [ST CASES]]]". *)
+  (*   iPoseProof (mytk_find_some with "[MYTK TKS]") as "%FIND". iFrame. *)
+  (*   iDestruct "CASES" as "[[%CT I] | [%CF [I | [I | I]]]]". *)
+  (*   { iPoseProof (locked_myturn with "MYTN I") as "%FF". eauto. inv FF. } *)
+  (*   { iPoseProof (unlocking_myturn with "MYTN I") as "%FF". eauto. inv FF. } *)
+  (*   { iPoseProof (unlocked0_contra with "I") as "%FF". eauto. inv FF. } *)
+  (*   iPoseProof (unlocked1_myturn with "MYTN I") as "%EQ". eauto. subst now. *)
 
-    unfold Mod.wrap_fun, WMem.load_fun. rred.
-    iDestruct "MEM" as "[MEM0 [MEM1 [MEM2 MEM3]]]". iDestruct "ST" as "[ST0 ST1]".
-    iApply stsim_getR. iSplit. eauto. rred.
-    iApply stsim_tauR. rred.
-    iPoseProof (memory_ra_load with "MEM0 MEM1") as "%LOAD". des. rewrite LOAD. rred.
-    iApply stsim_tauR. rred.
-    rewrite close_itree_call. rred.
+  (*   unfold Mod.wrap_fun, WMem.load_fun. rred. *)
+  (*   iDestruct "MEM" as "[MEM0 [MEM1 [MEM2 MEM3]]]". iDestruct "ST" as "[ST0 ST1]". *)
+  (*   iApply stsim_getR. iSplit. eauto. rred. *)
+  (*   iApply stsim_tauR. rred. *)
+  (*   iPoseProof (memory_ra_load with "MEM0 MEM1") as "%LOAD". des. rewrite LOAD. rred. *)
+  (*   iApply stsim_tauR. rred. *)
+  (*   rewrite close_itree_call. rred. *)
 
-    iMod ("K" with "[TKS MEM0 MEM1 MEM2 MEM3 ST0 ST1 I]") as "_".
-    { iExists mem, own, l, tks, mytk, next, myt. iFrame. iRight. iSplit; auto. }
-    clear pt mem own l tks next myt FIND CF LOAD LOAD0.
-    assert (exists tx0, tx = S tx0).
-    { inv TX; eauto. }
-    des. subst tx.
-    iApply lock_myturn_yieldR. iSplitL. iFrame. auto.
-    iIntros "[MYTK [MYNUM _]]". rred.
+  (*   iMod ("K" with "[TKS MEM0 MEM1 MEM2 MEM3 ST0 ST1 I]") as "_". *)
+  (*   { iExists mem, own, l, tks, mytk, next, myt. iFrame. iRight. iSplit; auto. } *)
+  (*   clear pt mem own l tks next myt FIND CF LOAD LOAD0. *)
+  (*   assert (exists tx0, tx = S tx0). *)
+  (*   { inv TX; eauto. } *)
+  (*   des. subst tx. *)
+  (*   iApply lock_myturn_yieldR. iSplitL. iFrame. auto. *)
+  (*   iIntros "[MYTK [MYNUM _]]". rred. *)
 
-    iopen 0 "I" "K". do 7 iDestruct "I" as "[% I]". iDestruct "I" as "[TKS [MEM [ST CASES]]]".
-    iPoseProof (mytk_find_some with "[MYTK TKS]") as "%FIND". iFrame.
-    iDestruct "CASES" as "[[%CT I] | [%CF [I | [I | I]]]]".
-    { iPoseProof (locked_myturn with "MYTN I") as "%FF". eauto. inv FF. }
-    { iPoseProof (unlocking_myturn with "MYTN I") as "%FF". eauto. inv FF. }
-    { iPoseProof (unlocked0_contra with "I") as "%FF". eauto. inv FF. }
-    iPoseProof (unlocked1_myturn with "MYTN I") as "%EQ". eauto. subst now.
+  (*   iopen 0 "I" "K". do 7 iDestruct "I" as "[% I]". iDestruct "I" as "[TKS [MEM [ST CASES]]]". *)
+  (*   iPoseProof (mytk_find_some with "[MYTK TKS]") as "%FIND". iFrame. *)
+  (*   iDestruct "CASES" as "[[%CT I] | [%CF [I | [I | I]]]]". *)
+  (*   { iPoseProof (locked_myturn with "MYTN I") as "%FF". eauto. inv FF. } *)
+  (*   { iPoseProof (unlocking_myturn with "MYTN I") as "%FF". eauto. inv FF. } *)
+  (*   { iPoseProof (unlocked0_contra with "I") as "%FF". eauto. inv FF. } *)
+  (*   iPoseProof (unlocked1_myturn with "MYTN I") as "%EQ". eauto. subst now. *)
 
-    unfold Mod.wrap_fun, WMem.compare_fun. rred.
-    iDestruct "MEM" as "[MEM0 [MEM1 [MEM2 MEM3]]]". iDestruct "ST" as "[ST0 ST1]".
-    iApply stsim_getR. iSplit. eauto. rred.
-    iApply stsim_tauR. rred. iApply stsim_tauR. rred.
-    destruct (Nat.eq_dec mytk mytk).
-    2:{ exfalso. auto. }
-    clear e. subst. rred.
+  (*   unfold Mod.wrap_fun, WMem.compare_fun. rred. *)
+  (*   iDestruct "MEM" as "[MEM0 [MEM1 [MEM2 MEM3]]]". iDestruct "ST" as "[ST0 ST1]". *)
+  (*   iApply stsim_getR. iSplit. eauto. rred. *)
+  (*   iApply stsim_tauR. rred. iApply stsim_tauR. rred. *)
+  (*   destruct (Nat.eq_dec mytk mytk). *)
+  (*   2:{ exfalso. auto. } *)
+  (*   clear e. subst. rred. *)
 
-    iApply stsim_yieldL. lred.
-    iApply stsim_getL. iSplit. auto. lred.
-    iApply stsim_getL. iSplit. auto.
-    iApply (stsim_putL with "ST1"). iIntros "ST1".
+  (*   iApply stsim_yieldL. lred. *)
+  (*   iApply stsim_getL. iSplit. auto. lred. *)
+  (*   iApply stsim_getL. iSplit. auto. *)
+  (*   iApply (stsim_putL with "ST1"). iIntros "ST1". *)
 
-    remember (NatMap.remove tid tks) as tks'.
-    rewrite <- key_set_pull_rm_eq. rewrite <- Heqtks'.
-    iAssert (ticket_lock_inv_state mem true tks')%I with "[ST0 ST1]" as "ST". iFrame.
-    iAssert (ticket_lock_inv_mem mem mytk next myt)%I with "[MEM0 MEM1 MEM2 MEM3]" as "MEM". iFrame.
-    iDestruct "TKS" as "[TKS0 [TKS1 [TKS2 TKS3]]]".
-    do 2 iDestruct "I" as "[% I]". iDestruct "I" as "[I0 [% [%I2 [I3 [I4 I5]]]]]".
-    do 3 iDestruct "I5" as "[% I5]". iDestruct "I5" as "[I5 [I6 [I7 [I8 [I9 I10]]]]]".
-    hexploit (tkqueue_inv_hd I2 _ FIND). i. des.
-    subst l. inversion H0; clear H0. subst yourt waits.
+  (*   remember (NatMap.remove tid tks) as tks'. *)
+  (*   rewrite <- key_set_pull_rm_eq. rewrite <- Heqtks'. *)
+  (*   iAssert (ticket_lock_inv_state mem true tks')%I with "[ST0 ST1]" as "ST". iFrame. *)
+  (*   iAssert (ticket_lock_inv_mem mem mytk next myt)%I with "[MEM0 MEM1 MEM2 MEM3]" as "MEM". iFrame. *)
+  (*   iDestruct "TKS" as "[TKS0 [TKS1 [TKS2 TKS3]]]". *)
+  (*   do 2 iDestruct "I" as "[% I]". iDestruct "I" as "[I0 [% [%I2 [I3 [I4 I5]]]]]". *)
+  (*   do 3 iDestruct "I5" as "[% I5]". iDestruct "I5" as "[I5 [I6 [I7 [I8 [I9 I10]]]]]". *)
+  (*   hexploit (tkqueue_inv_hd I2 _ FIND). i. des. *)
+  (*   subst l. inversion H0; clear H0. subst yourt waits. *)
 
-    iPoseProof (NatMapRA_remove with "TKS0 MYTK") as ">TKS0". rewrite <- Heqtks'.
-    iPoseProof (natmap_prop_remove_find with "TKS2") as "[MYTH TKS2]". eauto. rewrite <- Heqtks'.
-    iCombine "I10 MYNUM" as "MYNUM". rewrite maps_to_res_add.
-    iPoseProof (OwnM_Upd with "MYNUM") as "> MYNUM".
-    { eapply maps_to_updatable. apply Auth.auth_update.
-      instantiate (1:=Excl.just 0). instantiate (1:=Excl.just 0).
-      ii. des. ur in FRAME. des_ifs. split; ur; ss.
-    }
-    iPoseProof (OwnMs_fold with "[TKS3 MYNUM]") as "TKS3".
-    2:{ iSplitL "TKS3". iFrame. iFrame. }
-    { instantiate (1:= fun id => ~ NatMap.In id tks'). i. ss. subst tks'.
-      destruct (tid_dec j tid); auto. left. ii. apply IN.
-      rewrite NatMapP.F.remove_neq_in_iff; auto.
-    }
+  (*   iPoseProof (NatMapRA_remove with "TKS0 MYTK") as ">TKS0". rewrite <- Heqtks'. *)
+  (*   iPoseProof (natmap_prop_remove_find with "TKS2") as "[MYTH TKS2]". eauto. rewrite <- Heqtks'. *)
+  (*   iCombine "I10 MYNUM" as "MYNUM". rewrite maps_to_res_add. *)
+  (*   iPoseProof (OwnM_Upd with "MYNUM") as "> MYNUM". *)
+  (*   { eapply maps_to_updatable. apply Auth.auth_update. *)
+  (*     instantiate (1:=Excl.just 0). instantiate (1:=Excl.just 0). *)
+  (*     ii. des. ur in FRAME. des_ifs. split; ur; ss. *)
+  (*   } *)
+  (*   iPoseProof (OwnMs_fold with "[TKS3 MYNUM]") as "TKS3". *)
+  (*   2:{ iSplitL "TKS3". iFrame. iFrame. } *)
+  (*   { instantiate (1:= fun id => ~ NatMap.In id tks'). i. ss. subst tks'. *)
+  (*     destruct (tid_dec j tid); auto. left. ii. apply IN. *)
+  (*     rewrite NatMapP.F.remove_neq_in_iff; auto. *)
+  (*   } *)
 
-    iClear "I6 I9". iPoseProof (ObligationRA.pending_shot with "I7") as ">I7".
-    iPoseProof (ObligationRA.duty_done with "I8 I7") as ">DUTY".
-    iPoseProof (black_updatable with "I5") as ">I5".
-    { instantiate (1:=(mytk, Tkst.c k)). econs 2. ss. split; ss. lia. }
-    hexploit (tkqueue_dequeue I2).
-    { reflexivity. }
-    i. rename I2 into I2Old, H into I2. unfold TicketLockW.tk in I2. rewrite <- Heqtks' in I2.
-    iPoseProof (natmap_prop_remove with "I3") as "I3". rewrite <- Heqtks'.
+  (*   iClear "I6 I9". iPoseProof (ObligationRA.pending_shot with "I7") as ">I7". *)
+  (*   iPoseProof (ObligationRA.duty_done with "I8 I7") as ">DUTY". *)
+  (*   iPoseProof (black_updatable with "I5") as ">I5". *)
+  (*   { instantiate (1:=(mytk, Tkst.c k)). econs 2. ss. split; ss. lia. } *)
+  (*   hexploit (tkqueue_dequeue I2). *)
+  (*   { reflexivity. } *)
+  (*   i. rename I2 into I2Old, H into I2. unfold TicketLockW.tk in I2. rewrite <- Heqtks' in I2. *)
+  (*   iPoseProof (natmap_prop_remove with "I3") as "I3". rewrite <- Heqtks'. *)
 
-    iPoseProof (natmap_prop_sum_impl with "I3") as "I3".
-    { instantiate (1:= fun th tk =>
-                         ((FairRA.white th (Ord.from_nat (tk - (S mytk))))
-                            ∗ (FairRA.white th Ord.one))%I).
-      i. ss. iIntros "WHI". erewrite FairRA.white_eq.
-      2:{ instantiate (1:= (OrderedCM.add (Ord.from_nat (a - (S mytk))) (Ord.one))).
-          rewrite <- Ord.from_nat_1. ss. rewrite <- Hessenberg.add_from_nat. rr. ss.
-          hexploit (tkqueue_val_range_l I2 _ IN). i. split.
-          { apply OrdArith.le_from_nat. lia. }
-          { apply OrdArith.le_from_nat. lia. }
-      }
-      iPoseProof (FairRA.white_split with "WHI") as "[WHI1 WHI2]". iFrame.
-    }
-    iPoseProof (natmap_prop_sepconj_sum with "I3") as "[I3 TAX]".
+  (*   iPoseProof (natmap_prop_sum_impl with "I3") as "I3". *)
+  (*   { instantiate (1:= fun th tk => *)
+  (*                        ((FairRA.white th (Ord.from_nat (tk - (S mytk)))) *)
+  (*                           ∗ (FairRA.white th Ord.one))%I). *)
+  (*     i. ss. iIntros "WHI". erewrite FairRA.white_eq. *)
+  (*     2:{ instantiate (1:= (OrderedCM.add (Ord.from_nat (a - (S mytk))) (Ord.one))). *)
+  (*         rewrite <- Ord.from_nat_1. ss. rewrite <- Hessenberg.add_from_nat. rr. ss. *)
+  (*         hexploit (tkqueue_val_range_l I2 _ IN). i. split. *)
+  (*         { apply OrdArith.le_from_nat. lia. } *)
+  (*         { apply OrdArith.le_from_nat. lia. } *)
+  (*     } *)
+  (*     iPoseProof (FairRA.white_split with "WHI") as "[WHI1 WHI2]". iFrame. *)
+  (*   } *)
+  (*   iPoseProof (natmap_prop_sepconj_sum with "I3") as "[I3 TAX]". *)
 
-    iApply (stsim_fairL with "[TAX]").
-    { i. ss. instantiate (1:= (NatSet.elements (key_set tks'))). des_ifs. 
-      eapply NatSetIn_In. auto.
-    }
-    { instantiate (1:=[tid]). i; ss. des; clarify. des_ifs. }
-    { unfold natmap_prop_sum. unfold NatSet.elements. unfold nm_proj1.
-      unfold key_set. rewrite <- list_map_elements_nm_map. unfold unit1. rewrite List.map_map.
-      iPoseProof (list_prop_sum_map with "TAX") as "TAX".
-      2: iFrame.
-      ss. i. destruct a; ss.
-    }
-    instantiate (1:= Ord.omega). iIntros "[MYW _]".
-    iPoseProof (FairRA.whites_fold with "[TKS1 MYW]") as "TKS1".
-    2:{ iSplitL "TKS1". iFrame. iFrame. }
-    { instantiate (1:= fun id => ~ NatMap.In id tks'). ss. i. destruct (tid_dec j tid); auto.
-      left. ii. apply IN. subst tks'. rewrite NatMapP.F.remove_neq_in_iff; auto.
-    }
+  (*   iApply (stsim_fairL with "[TAX]"). *)
+  (*   { i. ss. instantiate (1:= (NatSet.elements (key_set tks'))). des_ifs.  *)
+  (*     eapply NatSetIn_In. auto. *)
+  (*   } *)
+  (*   { instantiate (1:=[tid]). i; ss. des; clarify. des_ifs. } *)
+  (*   { unfold natmap_prop_sum. unfold NatSet.elements. unfold nm_proj1. *)
+  (*     unfold key_set. rewrite <- list_map_elements_nm_map. unfold unit1. rewrite List.map_map. *)
+  (*     iPoseProof (list_prop_sum_map with "TAX") as "TAX". *)
+  (*     2: iFrame. *)
+  (*     ss. i. destruct a; ss. *)
+  (*   } *)
+  (*   instantiate (1:= Ord.omega). iIntros "[MYW _]". *)
+  (*   iPoseProof (FairRA.whites_fold with "[TKS1 MYW]") as "TKS1". *)
+  (*   2:{ iSplitL "TKS1". iFrame. iFrame. } *)
+  (*   { instantiate (1:= fun id => ~ NatMap.In id tks'). ss. i. destruct (tid_dec j tid); auto. *)
+  (*     left. ii. apply IN. subst tks'. rewrite NatMapP.F.remove_neq_in_iff; auto. *)
+  (*   } *)
 
-    iMod ("K" with "[I0 I4 ST MEM TKS0 TKS2 TKS3 I5 I3 TKS1]") as "_".
-    { iExists mem, true, tl, tks', mytk, next, myt.
-      remember 
-    ((⌜true = true⌝ ** ticket_lock_inv_locked tl tks' mytk next myt)
-    ∨ (⌜true = false⌝ **
-       ticket_lock_inv_unlocking tl tks' mytk next myt
-       ∨ ticket_lock_inv_unlocked0 tl tks' mytk next myt
-       ∨ ticket_lock_inv_unlocked1 tl tks' mytk next myt))%I as temp.
-      iFrame. subst temp. iLeft. iSplit. auto.
-      iFrame. iSplit. auto. iExists k. iFrame.
-    }
-    iApply (stsim_sync with "[DUTY]"). msubtac. iFrame.
-    iIntros "DUTY _". rred.
-    iApply stsim_tauR. iApply stsim_ret. iModIntro. iFrame. auto.
+  (*   iMod ("K" with "[I0 I4 ST MEM TKS0 TKS2 TKS3 I5 I3 TKS1]") as "_". *)
+  (*   { iExists mem, true, tl, tks', mytk, next, myt. *)
+  (*     remember  *)
+  (*   ((⌜true = true⌝ ** ticket_lock_inv_locked tl tks' mytk next myt) *)
+  (*   ∨ (⌜true = false⌝ ** *)
+  (*      ticket_lock_inv_unlocking tl tks' mytk next myt *)
+  (*      ∨ ticket_lock_inv_unlocked0 tl tks' mytk next myt *)
+  (*      ∨ ticket_lock_inv_unlocked1 tl tks' mytk next myt))%I as temp. *)
+  (*     iFrame. subst temp. iLeft. iSplit. auto. *)
+  (*     iFrame. iSplit. auto. iExists k. iFrame. *)
+  (*   } *)
+  (*   iApply (stsim_sync with "[DUTY]"). msubtac. iFrame. *)
+  (*   iIntros "DUTY _". rred. *)
+  (*   iApply stsim_tauR. iApply stsim_ret. iModIntro. iFrame. auto. *)
 
-  Qed.
+  (* Qed. *)
 
-  Lemma lock_myturn1
-        (g0 g1 : ∀ R_src R_tgt : Type,
-            (R_src → R_tgt → iProp)
-            → bool
-            → bool
-            → itree ((eventE +' cE) +' sE (Mod.state AbsLockW.mod)) R_src
-            → itree ((eventE +' cE) +' sE (OMod.closed_state TicketLock.omod (WMem.mod TicketLock.gvs))) R_tgt → iProp)
-        (ps pt: bool)
-        (tid : nat)
-        (mytk : TicketLockW.tk)
-        (mem : WMem.t)
-        (own : bool)
-        (l : list nat)
-        (tks : NatMap.t nat)
-        (next myt : nat)
-    :
-  (OwnM (Auth.white (NatMapRA.singleton tid mytk: NatMapRA.t nat)) **
-   (maps_to tid (Auth.white (Excl.just 2: Excl.t nat)) **
-    (ticket_lock_inv_tks tks **
-     (ticket_lock_inv_mem mem mytk next myt **
-      (ticket_lock_inv_state mem own tks **
-       ((⌜own = true⌝ ** ticket_lock_inv_locked l tks mytk next myt)
-        ∨ (⌜own = false⌝ **
-           ticket_lock_inv_unlocking l tks mytk next myt
-           ∨ ticket_lock_inv_unlocked0 l tks mytk next myt
-             ∨ ticket_lock_inv_unlocked1 l tks mytk next myt) **
-        (ticket_lock_inv -*
-         MUpd (nth_default True%I I)
-           (fairI (ident_tgt:=OMod.closed_ident TicketLock.omod (WMem.mod TicketLock.gvs))) []
-           [0] True)))))))
-  ⊢ (stsim I tid [] g0 g1
-      (λ r_src r_tgt : (), (own_thread tid ** ObligationRA.duty (inl tid) []) ** ⌜r_src = r_tgt⌝)
-      ps pt
-      (trigger Yield;;;
-       ` x : () + () <-
-       (` x_0 : bool * NatMap.t () <- trigger (Get (bool * NatMap.t ()));;
-        (let (own0, _) := x_0 in if Bool.eqb own0 true then Ret (inl ()) else Ret (inr ())));;
-       match x with
-       | inl l0 =>
-           tau;; ITree.iter
-                   (λ _ : (),
-                      trigger Yield;;;
-                      ` x_0 : bool * NatMap.t () <- trigger (Get (bool * NatMap.t ()));;
-                      (let (own0, _) := x_0 in
-                       if Bool.eqb own0 true then Ret (inl ()) else Ret (inr ()))) l0
-       | inr r0 => Ret r0
-       end;;;
-       ` x_0 : bool * NatMap.t () <- trigger (Get (bool * NatMap.t ()));;
-       (let (_, ts0) := x_0 in
-        trigger (Put (true, NatMap.remove (elt:=()) tid ts0));;;
-        trigger
-          (Fair
-             (λ i : nat,
-                if tid_dec i tid
-                then Flag.success
-                else
-                 if NatMapP.F.In_dec (NatMap.remove (elt:=()) tid ts0) i
-                 then Flag.fail
-                 else Flag.emp));;; trigger Yield;;; Ret ()))
-      (trigger Yield;;;
-       ` x : WMem.val <-
-       (` rv : Any.t <-
-        OMod.embed_itree TicketLock.omod (WMem.mod TicketLock.gvs)
-          (Mod.wrap_fun WMem.load_fun (Any.upcast TicketLock.now_serving));;
-        (tau;; unwrap (Any.downcast rv)));;
-       OMod.close_itree TicketLock.omod (WMem.mod TicketLock.gvs)
-         (` b : bool <- OMod.call "compare" (x, WMem.val_nat mytk);;
-          (if b then Ret () else tau;; TicketLock.lock_loop (WMem.val_nat mytk)));;;
-         OMod.close_itree TicketLock.omod (WMem.mod TicketLock.gvs) (trigger Yield))).
-  Proof.
-    iIntros "[MYTK [MYN [TKS [MEM [ST [CASES K]]]]]]".
-    iAssert (⌜NatMap.find tid tks = Some mytk⌝)%I as "%FIND".
-    { iDestruct "TKS" as "[TKS0 _]". iApply (NatMapRA_find_some with "TKS0 MYTK"). }
-    iDestruct "CASES" as "[[%CT I] | [%CF [I | [I | I]]]]".
-    { iPoseProof (locked_contra with "I") as "%F". eauto. inv F. }
-    { iPoseProof (unlocking_contra with "I") as "%F". eauto. inv F. }
-    { iPoseProof (unlocked0_contra with "I") as "%F". eauto. inv F. }
-    iPoseProof (unlocked1_mono with "I") as "[%TKQ #MYMW]".
-    iDestruct "MYMW" as "[% [% [MYMW _]]]".
-    iMod ("K" with "[TKS MEM ST I]") as "_".
-    { iExists mem, own, l, tks, mytk, next, myt. iFrame. iRight. iSplit; auto. }
-    iApply lock_myturn_yieldR. iSplitL. iFrame. auto.
-    iIntros "[MYTK [MYN _]]". rred.
-    iApply lock_myturn0. 2: iFrame; auto. lia.
-  Qed.
+  (* Lemma lock_myturn1 *)
+  (*       (g0 g1 : ∀ R_src R_tgt : Type, *)
+  (*           (R_src → R_tgt → iProp) *)
+  (*           → bool *)
+  (*           → bool *)
+  (*           → itree ((eventE +' cE) +' sE (Mod.state AbsLockW.mod)) R_src *)
+  (*           → itree ((eventE +' cE) +' sE (OMod.closed_state TicketLock.omod (WMem.mod TicketLock.gvs))) R_tgt → iProp) *)
+  (*       (ps pt: bool) *)
+  (*       (tid : nat) *)
+  (*       (mytk : TicketLockW.tk) *)
+  (*       (mem : WMem.t) *)
+  (*       (own : bool) *)
+  (*       (l : list nat) *)
+  (*       (tks : NatMap.t nat) *)
+  (*       (next myt : nat) *)
+  (*   : *)
+  (* (OwnM (Auth.white (NatMapRA.singleton tid mytk: NatMapRA.t nat)) ** *)
+  (*  (maps_to tid (Auth.white (Excl.just 2: Excl.t nat)) ** *)
+  (*   (ticket_lock_inv_tks tks ** *)
+  (*    (ticket_lock_inv_mem mem mytk next myt ** *)
+  (*     (ticket_lock_inv_state mem own tks ** *)
+  (*      ((⌜own = true⌝ ** ticket_lock_inv_locked l tks mytk next myt) *)
+  (*       ∨ (⌜own = false⌝ ** *)
+  (*          ticket_lock_inv_unlocking l tks mytk next myt *)
+  (*          ∨ ticket_lock_inv_unlocked0 l tks mytk next myt *)
+  (*            ∨ ticket_lock_inv_unlocked1 l tks mytk next myt) ** *)
+  (*       (ticket_lock_inv -* *)
+  (*        MUpd (nth_default True%I I) *)
+  (*          (fairI (ident_tgt:=OMod.closed_ident TicketLock.omod (WMem.mod TicketLock.gvs))) [] *)
+  (*          [0] True))))))) *)
+  (* ⊢ (stsim I tid [] g0 g1 *)
+  (*     (λ r_src r_tgt : (), (own_thread tid ** ObligationRA.duty (inl tid) []) ** ⌜r_src = r_tgt⌝) *)
+  (*     ps pt *)
+  (*     (trigger Yield;;; *)
+  (*      ` x : () + () <- *)
+  (*      (` x_0 : bool * NatMap.t () <- trigger (Get (bool * NatMap.t ()));; *)
+  (*       (let (own0, _) := x_0 in if Bool.eqb own0 true then Ret (inl ()) else Ret (inr ())));; *)
+  (*      match x with *)
+  (*      | inl l0 => *)
+  (*          tau;; ITree.iter *)
+  (*                  (λ _ : (), *)
+  (*                     trigger Yield;;; *)
+  (*                     ` x_0 : bool * NatMap.t () <- trigger (Get (bool * NatMap.t ()));; *)
+  (*                     (let (own0, _) := x_0 in *)
+  (*                      if Bool.eqb own0 true then Ret (inl ()) else Ret (inr ()))) l0 *)
+  (*      | inr r0 => Ret r0 *)
+  (*      end;;; *)
+  (*      ` x_0 : bool * NatMap.t () <- trigger (Get (bool * NatMap.t ()));; *)
+  (*      (let (_, ts0) := x_0 in *)
+  (*       trigger (Put (true, NatMap.remove (elt:=()) tid ts0));;; *)
+  (*       trigger *)
+  (*         (Fair *)
+  (*            (λ i : nat, *)
+  (*               if tid_dec i tid *)
+  (*               then Flag.success *)
+  (*               else *)
+  (*                if NatMapP.F.In_dec (NatMap.remove (elt:=()) tid ts0) i *)
+  (*                then Flag.fail *)
+  (*                else Flag.emp));;; trigger Yield;;; Ret ())) *)
+  (*     (trigger Yield;;; *)
+  (*      ` x : WMem.val <- *)
+  (*      (` rv : Any.t <- *)
+  (*       OMod.embed_itree TicketLock.omod (WMem.mod TicketLock.gvs) *)
+  (*         (Mod.wrap_fun WMem.load_fun (Any.upcast TicketLock.now_serving));; *)
+  (*       (tau;; unwrap (Any.downcast rv)));; *)
+  (*      OMod.close_itree TicketLock.omod (WMem.mod TicketLock.gvs) *)
+  (*        (` b : bool <- OMod.call "compare" (x, WMem.val_nat mytk);; *)
+  (*         (if b then Ret () else tau;; TicketLock.lock_loop (WMem.val_nat mytk)));;; *)
+  (*        OMod.close_itree TicketLock.omod (WMem.mod TicketLock.gvs) (trigger Yield))). *)
+  (* Proof. *)
+  (*   iIntros "[MYTK [MYN [TKS [MEM [ST [CASES K]]]]]]". *)
+  (*   iAssert (⌜NatMap.find tid tks = Some mytk⌝)%I as "%FIND". *)
+  (*   { iDestruct "TKS" as "[TKS0 _]". iApply (NatMapRA_find_some with "TKS0 MYTK"). } *)
+  (*   iDestruct "CASES" as "[[%CT I] | [%CF [I | [I | I]]]]". *)
+  (*   { iPoseProof (locked_contra with "I") as "%F". eauto. inv F. } *)
+  (*   { iPoseProof (unlocking_contra with "I") as "%F". eauto. inv F. } *)
+  (*   { iPoseProof (unlocked0_contra with "I") as "%F". eauto. inv F. } *)
+  (*   iPoseProof (unlocked1_mono with "I") as "[%TKQ #MYMW]". *)
+  (*   iDestruct "MYMW" as "[% [% [MYMW _]]]". *)
+  (*   iMod ("K" with "[TKS MEM ST I]") as "_". *)
+  (*   { iExists mem, own, l, tks, mytk, next, myt. iFrame. iRight. iSplit; auto. } *)
+  (*   iApply lock_myturn_yieldR. iSplitL. iFrame. auto. *)
+  (*   iIntros "[MYTK [MYN _]]". rred. *)
+  (*   iApply lock_myturn0. 2: iFrame; auto. lia. *)
+  (* Qed. *)
 
-  Lemma lock_myturn2
-        (g0 g1 : ∀ R_src R_tgt : Type,
-            (R_src → R_tgt → iProp)
-            → bool
-            → bool
-            → itree ((eventE +' cE) +' sE (Mod.state AbsLockW.mod)) R_src
-            → itree ((eventE +' cE) +' sE (OMod.closed_state TicketLock.omod (WMem.mod TicketLock.gvs))) R_tgt → iProp)
-        (ps pt: bool)
-        (tid : nat)
-        (mytk : TicketLockW.tk)
-        (mem : WMem.t)
-        (own : bool)
-        (l : list nat)
-        (tks : NatMap.t nat)
-        (next myt : nat)
-        now_old
-        (NEQ: mytk <> now_old)
-    :
-  (OwnM (Auth.white (NatMapRA.singleton tid mytk: NatMapRA.t nat)) **
-   (maps_to tid (Auth.white (Excl.just 2: Excl.t nat)) **
-    (ticket_lock_inv_tks tks **
-     (ticket_lock_inv_mem mem mytk next myt **
-      (ticket_lock_inv_state mem own tks **
-       ((⌜own = true⌝ ** ticket_lock_inv_locked l tks mytk next myt)
-        ∨ (⌜own = false⌝ **
-           ticket_lock_inv_unlocking l tks mytk next myt
-           ∨ ticket_lock_inv_unlocked0 l tks mytk next myt
-             ∨ ticket_lock_inv_unlocked1 l tks mytk next myt) **
-        (ticket_lock_inv -*
-         MUpd (nth_default True%I I)
-           (fairI (ident_tgt:=OMod.closed_ident TicketLock.omod (WMem.mod TicketLock.gvs))) []
-           [0] True)))))))
-  ⊢ (stsim I tid [] g0 g1
-    (λ r_src r_tgt : (), (own_thread tid ** ObligationRA.duty (inl tid) []) ** ⌜r_src = r_tgt⌝)
-    ps pt
-    (trigger Yield;;;
-     ` x : () + () <-
-     (` x_0 : bool * NatMap.t () <- trigger (Get (bool * NatMap.t ()));;
-      (let (own0, _) := x_0 in if Bool.eqb own0 true then Ret (inl ()) else Ret (inr ())));;
-     match x with
-     | inl l0 =>
-         tau;; ITree.iter
-                 (λ _ : (),
-                    trigger Yield;;;
-                    ` x_0 : bool * NatMap.t () <- trigger (Get (bool * NatMap.t ()));;
-                    (let (own0, _) := x_0 in
-                     if Bool.eqb own0 true then Ret (inl ()) else Ret (inr ()))) l0
-     | inr r0 => Ret r0
-     end;;;
-     ` x_0 : bool * NatMap.t () <- trigger (Get (bool * NatMap.t ()));;
-     (let (_, ts0) := x_0 in
-      trigger (Put (true, NatMap.remove (elt:=()) tid ts0));;;
-      trigger
-        (Fair
-           (λ i : nat,
-              if tid_dec i tid
-              then Flag.success
-              else
-               if NatMapP.F.In_dec (NatMap.remove (elt:=()) tid ts0) i
-               then Flag.fail
-               else Flag.emp));;; trigger Yield;;; Ret ()))
-    (` r : Any.t <-
-     OMod.embed_itree TicketLock.omod (WMem.mod TicketLock.gvs)
-       (Mod.wrap_fun WMem.compare_fun (Any.upcast (WMem.val_nat now_old, WMem.val_nat mytk)));;
-     ` x : bool <- (tau;; unwrap (Any.downcast r));;
-     OMod.close_itree TicketLock.omod (WMem.mod TicketLock.gvs)
-       (if x then Ret () else tau;; TicketLock.lock_loop (WMem.val_nat mytk));;;
-       OMod.close_itree TicketLock.omod (WMem.mod TicketLock.gvs) (trigger Yield))).
-  Proof.
-    iIntros "[MYTK [MYN [TKS [MEM [ST [CASES K]]]]]]".
-    unfold Mod.wrap_fun, WMem.compare_fun. rred.
-    iDestruct "MEM" as "[MEM0 [MEM1 [MEM2 MEM3]]]". iDestruct "ST" as "[ST0 ST1]".
-    iApply stsim_getR. iSplit. eauto. rred.
-    iApply stsim_tauR. rred. iApply stsim_tauR. rred.
-    destruct (Nat.eq_dec now_old mytk).
-    { exfalso. clarify. }
-    rred. iApply stsim_tauR.
-    rewrite TicketLock.lock_loop_red. rred. rewrite close_itree_call. rred.
-    iApply lock_myturn1.
-    iSplitL "MYTK". iFrame. iSplitL "MYN". iFrame. iSplitL "TKS". iFrame.
-    iSplitL "MEM0 MEM1 MEM2 MEM3". iFrame. iSplitL "ST0 ST1". iFrame. iSplitL "CASES". iFrame.
-    iFrame.
-  Qed.
+  (* Lemma lock_myturn2 *)
+  (*       (g0 g1 : ∀ R_src R_tgt : Type, *)
+  (*           (R_src → R_tgt → iProp) *)
+  (*           → bool *)
+  (*           → bool *)
+  (*           → itree ((eventE +' cE) +' sE (Mod.state AbsLockW.mod)) R_src *)
+  (*           → itree ((eventE +' cE) +' sE (OMod.closed_state TicketLock.omod (WMem.mod TicketLock.gvs))) R_tgt → iProp) *)
+  (*       (ps pt: bool) *)
+  (*       (tid : nat) *)
+  (*       (mytk : TicketLockW.tk) *)
+  (*       (mem : WMem.t) *)
+  (*       (own : bool) *)
+  (*       (l : list nat) *)
+  (*       (tks : NatMap.t nat) *)
+  (*       (next myt : nat) *)
+  (*       now_old *)
+  (*       (NEQ: mytk <> now_old) *)
+  (*   : *)
+  (* (OwnM (Auth.white (NatMapRA.singleton tid mytk: NatMapRA.t nat)) ** *)
+  (*  (maps_to tid (Auth.white (Excl.just 2: Excl.t nat)) ** *)
+  (*   (ticket_lock_inv_tks tks ** *)
+  (*    (ticket_lock_inv_mem mem mytk next myt ** *)
+  (*     (ticket_lock_inv_state mem own tks ** *)
+  (*      ((⌜own = true⌝ ** ticket_lock_inv_locked l tks mytk next myt) *)
+  (*       ∨ (⌜own = false⌝ ** *)
+  (*          ticket_lock_inv_unlocking l tks mytk next myt *)
+  (*          ∨ ticket_lock_inv_unlocked0 l tks mytk next myt *)
+  (*            ∨ ticket_lock_inv_unlocked1 l tks mytk next myt) ** *)
+  (*       (ticket_lock_inv -* *)
+  (*        MUpd (nth_default True%I I) *)
+  (*          (fairI (ident_tgt:=OMod.closed_ident TicketLock.omod (WMem.mod TicketLock.gvs))) [] *)
+  (*          [0] True))))))) *)
+  (* ⊢ (stsim I tid [] g0 g1 *)
+  (*   (λ r_src r_tgt : (), (own_thread tid ** ObligationRA.duty (inl tid) []) ** ⌜r_src = r_tgt⌝) *)
+  (*   ps pt *)
+  (*   (trigger Yield;;; *)
+  (*    ` x : () + () <- *)
+  (*    (` x_0 : bool * NatMap.t () <- trigger (Get (bool * NatMap.t ()));; *)
+  (*     (let (own0, _) := x_0 in if Bool.eqb own0 true then Ret (inl ()) else Ret (inr ())));; *)
+  (*    match x with *)
+  (*    | inl l0 => *)
+  (*        tau;; ITree.iter *)
+  (*                (λ _ : (), *)
+  (*                   trigger Yield;;; *)
+  (*                   ` x_0 : bool * NatMap.t () <- trigger (Get (bool * NatMap.t ()));; *)
+  (*                   (let (own0, _) := x_0 in *)
+  (*                    if Bool.eqb own0 true then Ret (inl ()) else Ret (inr ()))) l0 *)
+  (*    | inr r0 => Ret r0 *)
+  (*    end;;; *)
+  (*    ` x_0 : bool * NatMap.t () <- trigger (Get (bool * NatMap.t ()));; *)
+  (*    (let (_, ts0) := x_0 in *)
+  (*     trigger (Put (true, NatMap.remove (elt:=()) tid ts0));;; *)
+  (*     trigger *)
+  (*       (Fair *)
+  (*          (λ i : nat, *)
+  (*             if tid_dec i tid *)
+  (*             then Flag.success *)
+  (*             else *)
+  (*              if NatMapP.F.In_dec (NatMap.remove (elt:=()) tid ts0) i *)
+  (*              then Flag.fail *)
+  (*              else Flag.emp));;; trigger Yield;;; Ret ())) *)
+  (*   (` r : Any.t <- *)
+  (*    OMod.embed_itree TicketLock.omod (WMem.mod TicketLock.gvs) *)
+  (*      (Mod.wrap_fun WMem.compare_fun (Any.upcast (WMem.val_nat now_old, WMem.val_nat mytk)));; *)
+  (*    ` x : bool <- (tau;; unwrap (Any.downcast r));; *)
+  (*    OMod.close_itree TicketLock.omod (WMem.mod TicketLock.gvs) *)
+  (*      (if x then Ret () else tau;; TicketLock.lock_loop (WMem.val_nat mytk));;; *)
+  (*      OMod.close_itree TicketLock.omod (WMem.mod TicketLock.gvs) (trigger Yield))). *)
+  (* Proof. *)
+  (*   iIntros "[MYTK [MYN [TKS [MEM [ST [CASES K]]]]]]". *)
+  (*   unfold Mod.wrap_fun, WMem.compare_fun. rred. *)
+  (*   iDestruct "MEM" as "[MEM0 [MEM1 [MEM2 MEM3]]]". iDestruct "ST" as "[ST0 ST1]". *)
+  (*   iApply stsim_getR. iSplit. eauto. rred. *)
+  (*   iApply stsim_tauR. rred. iApply stsim_tauR. rred. *)
+  (*   destruct (Nat.eq_dec now_old mytk). *)
+  (*   { exfalso. clarify. } *)
+  (*   rred. iApply stsim_tauR. *)
+  (*   rewrite TicketLock.lock_loop_red. rred. rewrite close_itree_call. rred. *)
+  (*   iApply lock_myturn1. *)
+  (*   iSplitL "MYTK". iFrame. iSplitL "MYN". iFrame. iSplitL "TKS". iFrame. *)
+  (*   iSplitL "MEM0 MEM1 MEM2 MEM3". iFrame. iSplitL "ST0 ST1". iFrame. iSplitL "CASES". iFrame. *)
+  (*   iFrame. *)
+  (* Qed. *)
 
-  Let src_code_coind tid: itree ((eventE +' cE) +' sE (Mod.state AbsLockW.mod)) () :=
-          ((` lr : () + () <-
-            (trigger Yield;;;
-             ` x_0 : bool * NatMap.t () <- trigger (Get (bool * NatMap.t ()));;
-             (let (own0, _) := x_0 in if Bool.eqb own0 true then Ret (inl ()) else Ret (inr ())));;
-            match lr with
-            | inl l0 =>
-                tau;; ITree.iter
-                        (λ _ : (),
-                           trigger Yield;;;
-                           ` x_0 : bool * NatMap.t () <- trigger (Get (bool * NatMap.t ()));;
-                           (let (own0, _) := x_0 in
-                            if Bool.eqb own0 true then Ret (inl ()) else Ret (inr ()))) l0
-            | inr r0 => Ret r0
-            end);;;
-           ` x_0 : bool * NatMap.t () <- trigger (Get (bool * NatMap.t ()));;
-           (let (_, ts0) := x_0 in
-            trigger (Put (true, NatMap.remove (elt:=()) tid ts0));;;
-            trigger
-              (Fair
-                 (λ i : nat,
-                    if tid_dec i tid
-                    then Flag.success
-                    else
-                     if NatMapP.F.In_dec (NatMap.remove (elt:=()) tid ts0) i
-                     then Flag.fail
-                     else Flag.emp));;; trigger Yield;;; Ret ())).
+  (* Let src_code_coind tid: itree ((eventE +' cE) +' sE (Mod.state AbsLockW.mod)) () := *)
+  (*         ((` lr : () + () <- *)
+  (*           (trigger Yield;;; *)
+  (*            ` x_0 : bool * NatMap.t () <- trigger (Get (bool * NatMap.t ()));; *)
+  (*            (let (own0, _) := x_0 in if Bool.eqb own0 true then Ret (inl ()) else Ret (inr ())));; *)
+  (*           match lr with *)
+  (*           | inl l0 => *)
+  (*               tau;; ITree.iter *)
+  (*                       (λ _ : (), *)
+  (*                          trigger Yield;;; *)
+  (*                          ` x_0 : bool * NatMap.t () <- trigger (Get (bool * NatMap.t ()));; *)
+  (*                          (let (own0, _) := x_0 in *)
+  (*                           if Bool.eqb own0 true then Ret (inl ()) else Ret (inr ()))) l0 *)
+  (*           | inr r0 => Ret r0 *)
+  (*           end);;; *)
+  (*          ` x_0 : bool * NatMap.t () <- trigger (Get (bool * NatMap.t ()));; *)
+  (*          (let (_, ts0) := x_0 in *)
+  (*           trigger (Put (true, NatMap.remove (elt:=()) tid ts0));;; *)
+  (*           trigger *)
+  (*             (Fair *)
+  (*                (λ i : nat, *)
+  (*                   if tid_dec i tid *)
+  (*                   then Flag.success *)
+  (*                   else *)
+  (*                    if NatMapP.F.In_dec (NatMap.remove (elt:=()) tid ts0) i *)
+  (*                    then Flag.fail *)
+  (*                    else Flag.emp));;; trigger Yield;;; Ret ())). *)
 
-  Let tgt_code_coind a :=
-          (trigger Yield;;;
-           ` x : WMem.val <-
-           (` rv : Any.t <-
-            OMod.embed_itree TicketLock.omod (WMem.mod TicketLock.gvs)
-              (` arg : WMem.val <- unwrap (Any.downcast (Any.upcast TicketLock.now_serving));;
-               ` ret : WMem.val <-
-               (` m : WMem.t <- trigger (Get WMem.t);;
-                ` v : WMem.val <- unwrap (WMem.load m arg);; Ret v);; 
-               Ret (Any.upcast ret));; (tau;; unwrap (Any.downcast rv)));;
-           OMod.close_itree TicketLock.omod (WMem.mod TicketLock.gvs)
-             (` b : bool <- OMod.call "compare" (x, WMem.val_nat a);;
-              (if b then Ret () else tau;; TicketLock.lock_loop (WMem.val_nat a)));;;
-           OMod.close_itree TicketLock.omod (WMem.mod TicketLock.gvs) (trigger Yield)).
+  (* Let tgt_code_coind a := *)
+  (*         (trigger Yield;;; *)
+  (*          ` x : WMem.val <- *)
+  (*          (` rv : Any.t <- *)
+  (*           OMod.embed_itree TicketLock.omod (WMem.mod TicketLock.gvs) *)
+  (*             (` arg : WMem.val <- unwrap (Any.downcast (Any.upcast TicketLock.now_serving));; *)
+  (*              ` ret : WMem.val <- *)
+  (*              (` m : WMem.t <- trigger (Get WMem.t);; *)
+  (*               ` v : WMem.val <- unwrap (WMem.load m arg);; Ret v);;  *)
+  (*              Ret (Any.upcast ret));; (tau;; unwrap (Any.downcast rv)));; *)
+  (*          OMod.close_itree TicketLock.omod (WMem.mod TicketLock.gvs) *)
+  (*            (` b : bool <- OMod.call "compare" (x, WMem.val_nat a);; *)
+  (*             (if b then Ret () else tau;; TicketLock.lock_loop (WMem.val_nat a)));;; *)
+  (*          OMod.close_itree TicketLock.omod (WMem.mod TicketLock.gvs) (trigger Yield)). *)
 
-  Lemma lock_yourturn_coind
-        (g0 g1 : ∀ R_src R_tgt : Type,
-            (R_src → R_tgt → iProp)
-            → bool
-            → bool
-            → itree ((eventE +' cE) +' sE (Mod.state AbsLockW.mod)) R_src
-            → itree ((eventE +' cE) +' sE (OMod.closed_state TicketLock.omod (WMem.mod TicketLock.gvs))) R_tgt → iProp)
-        (ps pt: bool)
-        (tid : nat)
-        (mytk : TicketLockW.tk)
-        (mem : WMem.t)
-        (l : list nat)
-        (tks : NatMap.t nat)
-        (now next myt : nat)
-        now_old
-        (NEQ: mytk <> now_old)
-    :
-  (□ (∀ a : TicketLockW.tk,
-        (OwnM (Auth.white (NatMapRA.singleton tid a: NatMapRA.t nat)) ** maps_to tid (Auth.white (Excl.just 2: Excl.t nat))) -*
-        g1 ()%type ()%type
-          (λ r_src r_tgt : (),
-              (own_thread tid ** ObligationRA.duty (inl tid) []) ** ⌜r_src = r_tgt⌝) false false
-          (src_code_coind tid)
-          (tgt_code_coind a)
-     ) **
-   (maps_to tid (Auth.white (Excl.just 2: Excl.t nat)) **
-    (OwnM (Auth.white (NatMapRA.singleton tid mytk: NatMapRA.t nat)) **
-     (ticket_lock_inv_tks tks **
-      (ticket_lock_inv_mem mem now next myt **
-       (ticket_lock_inv_state mem true tks **
-        (ticket_lock_inv_locked l tks now next myt **
-         (ticket_lock_inv -*
-          MUpd (nth_default True%I I)
-            (fairI (ident_tgt:=OMod.closed_ident TicketLock.omod (WMem.mod TicketLock.gvs))) []
-            [0] True)))))))
-  )
-  ⊢ (stsim I tid [] g0 g1
-      (λ r_src r_tgt : (), (own_thread tid ** ObligationRA.duty (inl tid) []) ** ⌜r_src = r_tgt⌝)
-      ps pt
-      (trigger Yield;;;
-       ` x : () + () <-
-       (` x_0 : bool * NatMap.t () <- trigger (Get (bool * NatMap.t ()));;
-        (let (own0, _) := x_0 in if Bool.eqb own0 true then Ret (inl ()) else Ret (inr ())));;
-       match x with
-       | inl l0 =>
-           tau;; ITree.iter
-                   (λ _ : (),
-                      trigger Yield;;;
-                      ` x_0 : bool * NatMap.t () <- trigger (Get (bool * NatMap.t ()));;
-                      (let (own0, _) := x_0 in
-                       if Bool.eqb own0 true then Ret (inl ()) else Ret (inr ()))) l0
-       | inr r0 => Ret r0
-       end;;;
-       ` x_0 : bool * NatMap.t () <- trigger (Get (bool * NatMap.t ()));;
-       (let (_, ts0) := x_0 in
-        trigger (Put (true, NatMap.remove (elt:=()) tid ts0));;;
-        trigger
-          (Fair
-             (λ i : nat,
-                if tid_dec i tid
-                then Flag.success
-                else
-                 if NatMapP.F.In_dec (NatMap.remove (elt:=()) tid ts0) i
-                 then Flag.fail
-                 else Flag.emp));;; trigger Yield;;; Ret ()))
-      (` r : Any.t <-
-       OMod.embed_itree TicketLock.omod (WMem.mod TicketLock.gvs)
-         (Mod.wrap_fun WMem.compare_fun (Any.upcast (WMem.val_nat now_old, WMem.val_nat mytk)));;
-       ` x : bool <- (tau;; unwrap (Any.downcast r));;
-       OMod.close_itree TicketLock.omod (WMem.mod TicketLock.gvs)
-         (if x then Ret () else tau;; TicketLock.lock_loop (WMem.val_nat mytk));;;
-       OMod.close_itree TicketLock.omod (WMem.mod TicketLock.gvs) (trigger Yield))).
-  Proof.
-    iIntros "[#CIH [MYTK [MYN [TKS [MEM [ST [I K]]]]]]]".
-    unfold Mod.wrap_fun, WMem.compare_fun. rred.
-    iDestruct "MEM" as "[MEM0 [MEM1 [MEM2 MEM3]]]". iDestruct "ST" as "[ST0 ST1]".
-    iApply stsim_getR. iSplit. eauto. rred.
-    iApply stsim_tauR. rred. iApply stsim_tauR. rred.
-    destruct (Nat.eq_dec now_old mytk).
-    { exfalso. clarify. }
-    rred. iApply stsim_tauR.
-    rewrite TicketLock.lock_loop_red. rred. rewrite close_itree_call. rred.
+  (* Lemma lock_yourturn_coind *)
+  (*       (g0 g1 : ∀ R_src R_tgt : Type, *)
+  (*           (R_src → R_tgt → iProp) *)
+  (*           → bool *)
+  (*           → bool *)
+  (*           → itree ((eventE +' cE) +' sE (Mod.state AbsLockW.mod)) R_src *)
+  (*           → itree ((eventE +' cE) +' sE (OMod.closed_state TicketLock.omod (WMem.mod TicketLock.gvs))) R_tgt → iProp) *)
+  (*       (ps pt: bool) *)
+  (*       (tid : nat) *)
+  (*       (mytk : TicketLockW.tk) *)
+  (*       (mem : WMem.t) *)
+  (*       (l : list nat) *)
+  (*       (tks : NatMap.t nat) *)
+  (*       (now next myt : nat) *)
+  (*       now_old *)
+  (*       (NEQ: mytk <> now_old) *)
+  (*   : *)
+  (* (□ (∀ a : TicketLockW.tk, *)
+  (*       (OwnM (Auth.white (NatMapRA.singleton tid a: NatMapRA.t nat)) ** maps_to tid (Auth.white (Excl.just 2: Excl.t nat))) -* *)
+  (*       g1 ()%type ()%type *)
+  (*         (λ r_src r_tgt : (), *)
+  (*             (own_thread tid ** ObligationRA.duty (inl tid) []) ** ⌜r_src = r_tgt⌝) false false *)
+  (*         (src_code_coind tid) *)
+  (*         (tgt_code_coind a) *)
+  (*    ) ** *)
+  (*  (maps_to tid (Auth.white (Excl.just 2: Excl.t nat)) ** *)
+  (*   (OwnM (Auth.white (NatMapRA.singleton tid mytk: NatMapRA.t nat)) ** *)
+  (*    (ticket_lock_inv_tks tks ** *)
+  (*     (ticket_lock_inv_mem mem now next myt ** *)
+  (*      (ticket_lock_inv_state mem true tks ** *)
+  (*       (ticket_lock_inv_locked l tks now next myt ** *)
+  (*        (ticket_lock_inv -* *)
+  (*         MUpd (nth_default True%I I) *)
+  (*           (fairI (ident_tgt:=OMod.closed_ident TicketLock.omod (WMem.mod TicketLock.gvs))) [] *)
+  (*           [0] True))))))) *)
+  (* ) *)
+  (* ⊢ (stsim I tid [] g0 g1 *)
+  (*     (λ r_src r_tgt : (), (own_thread tid ** ObligationRA.duty (inl tid) []) ** ⌜r_src = r_tgt⌝) *)
+  (*     ps pt *)
+  (*     (trigger Yield;;; *)
+  (*      ` x : () + () <- *)
+  (*      (` x_0 : bool * NatMap.t () <- trigger (Get (bool * NatMap.t ()));; *)
+  (*       (let (own0, _) := x_0 in if Bool.eqb own0 true then Ret (inl ()) else Ret (inr ())));; *)
+  (*      match x with *)
+  (*      | inl l0 => *)
+  (*          tau;; ITree.iter *)
+  (*                  (λ _ : (), *)
+  (*                     trigger Yield;;; *)
+  (*                     ` x_0 : bool * NatMap.t () <- trigger (Get (bool * NatMap.t ()));; *)
+  (*                     (let (own0, _) := x_0 in *)
+  (*                      if Bool.eqb own0 true then Ret (inl ()) else Ret (inr ()))) l0 *)
+  (*      | inr r0 => Ret r0 *)
+  (*      end;;; *)
+  (*      ` x_0 : bool * NatMap.t () <- trigger (Get (bool * NatMap.t ()));; *)
+  (*      (let (_, ts0) := x_0 in *)
+  (*       trigger (Put (true, NatMap.remove (elt:=()) tid ts0));;; *)
+  (*       trigger *)
+  (*         (Fair *)
+  (*            (λ i : nat, *)
+  (*               if tid_dec i tid *)
+  (*               then Flag.success *)
+  (*               else *)
+  (*                if NatMapP.F.In_dec (NatMap.remove (elt:=()) tid ts0) i *)
+  (*                then Flag.fail *)
+  (*                else Flag.emp));;; trigger Yield;;; Ret ())) *)
+  (*     (` r : Any.t <- *)
+  (*      OMod.embed_itree TicketLock.omod (WMem.mod TicketLock.gvs) *)
+  (*        (Mod.wrap_fun WMem.compare_fun (Any.upcast (WMem.val_nat now_old, WMem.val_nat mytk)));; *)
+  (*      ` x : bool <- (tau;; unwrap (Any.downcast r));; *)
+  (*      OMod.close_itree TicketLock.omod (WMem.mod TicketLock.gvs) *)
+  (*        (if x then Ret () else tau;; TicketLock.lock_loop (WMem.val_nat mytk));;; *)
+  (*      OMod.close_itree TicketLock.omod (WMem.mod TicketLock.gvs) (trigger Yield))). *)
+  (* Proof. *)
+  (*   iIntros "[#CIH [MYTK [MYN [TKS [MEM [ST [I K]]]]]]]". *)
+  (*   unfold Mod.wrap_fun, WMem.compare_fun. rred. *)
+  (*   iDestruct "MEM" as "[MEM0 [MEM1 [MEM2 MEM3]]]". iDestruct "ST" as "[ST0 ST1]". *)
+  (*   iApply stsim_getR. iSplit. eauto. rred. *)
+  (*   iApply stsim_tauR. rred. iApply stsim_tauR. rred. *)
+  (*   destruct (Nat.eq_dec now_old mytk). *)
+  (*   { exfalso. clarify. } *)
+  (*   rred. iApply stsim_tauR. *)
+  (*   rewrite TicketLock.lock_loop_red. rred. rewrite close_itree_call. rred. *)
 
-    iApply stsim_yieldL. lred.
-    iApply stsim_getL. iSplit. auto. lred.
-    iApply stsim_tauL.
-    iMod ("K" with "[TKS MEM0 MEM1 MEM2 MEM3 ST0 ST1 I]") as "_".
-    { do 7 iExists _.
-      iSplitL "TKS". iFrame. iSplitL "MEM0 MEM1 MEM2 MEM3". iFrame.
-      iSplitL "ST0 ST1". iFrame.
-      iLeft. iSplit. auto. iFrame.
-    }
-    iApply stsim_progress. iApply stsim_base. msubtac.
-    rewrite unfold_iter_eq. iApply "CIH". iFrame.
-  Qed.
+  (*   iApply stsim_yieldL. lred. *)
+  (*   iApply stsim_getL. iSplit. auto. lred. *)
+  (*   iApply stsim_tauL. *)
+  (*   iMod ("K" with "[TKS MEM0 MEM1 MEM2 MEM3 ST0 ST1 I]") as "_". *)
+  (*   { do 7 iExists _. *)
+  (*     iSplitL "TKS". iFrame. iSplitL "MEM0 MEM1 MEM2 MEM3". iFrame. *)
+  (*     iSplitL "ST0 ST1". iFrame. *)
+  (*     iLeft. iSplit. auto. iFrame. *)
+  (*   } *)
+  (*   iApply stsim_progress. iApply stsim_base. msubtac. *)
+  (*   rewrite unfold_iter_eq. iApply "CIH". iFrame. *)
+  (* Qed. *)
 
   Lemma yourturn_range
-        tid tks mytk now next own l myt
+        tid tks mytk now next own ing l myt V
         (FIND : NatMap.find tid tks = Some mytk)
         (NEQ : mytk ≠ now)
     :
-    ((⌜own = true⌝ ∗ ticket_lock_inv_locked l tks now next myt)
-     ∨ (⌜own = false⌝ ∗
-                    (ticket_lock_inv_unlocking l tks now next myt
-                     ∨ ticket_lock_inv_unlocked0 l tks now next myt
-                     ∨ ticket_lock_inv_unlocked1 l tks now next myt)))
-      ⊢
+    ((⌜own = true⌝ ∗
+     ((⌜ing = false⌝ ∗ ticket_lock_inv_locked l tks now next myt V) ∨ (⌜ing = true⌝ ∗ ticket_lock_inv_unlocking l tks now next myt)))
+    ∨ (⌜own = false⌝ ∗
+                   (⌜ing = false⌝ ∗
+                                (ticket_lock_inv_unlocked0 l tks now next myt V ∨ ticket_lock_inv_unlocked1 l tks now next myt V))))
+        ⊢
       (⌜now < mytk⌝).
   Proof.
-    iIntros "[[%CT I] | [%CF [I | [I | I]]]]".
+    iIntros "[[%CT [[%IF I] | [%IT I]]] | [%CF [%IF [I | I]]]]".
     { iDestruct "I" as "[_ [%I1 _]]".
       hexploit (tkqueue_val_range_l I1 _ FIND). i. iPureIntro. lia. }
     { iDestruct "I" as "[_ [%I1 _]]".
@@ -1540,593 +1599,593 @@ Section SIM.
       hexploit (tkqueue_val_range_l I1 _ FIND). i. iPureIntro. lia. }
   Qed.
 
-  Let src_code_ind tid: itree ((eventE +' cE) +' sE (Mod.state AbsLockW.mod)) () :=
-                         (trigger Yield;;;
-                          ` x : () + () <-
-                          (` x_0 : bool * NatMap.t () <- trigger (Get (bool * NatMap.t ()));;
-                           (let (own0, _) := x_0 in
-                            if Bool.eqb own0 true then Ret (inl ()) else Ret (inr ())));;
-                          match x with
-                          | inl l0 =>
-                              tau;; ITree.iter
-                                      (λ _ : (),
-                                         trigger Yield;;;
-                                         ` x_0 : bool * NatMap.t () <-
-                                         trigger (Get (bool * NatMap.t ()));;
-                                         (let (own0, _) := x_0 in
-                                          if Bool.eqb own0 true
-                                          then Ret (inl ())
-                                          else Ret (inr ()))) l0
-                          | inr r0 => Ret r0
-                          end;;;
-                          ` x_0 : bool * NatMap.t () <- trigger (Get (bool * NatMap.t ()));;
-                          (let (_, ts0) := x_0 in
-                           trigger (Put (true, NatMap.remove (elt:=()) tid ts0));;;
-                           trigger
-                             (Fair
-                                (λ i : nat,
-                                   if tid_dec i tid
-                                   then Flag.success
-                                   else
-                                    if NatMapP.F.In_dec (NatMap.remove (elt:=()) tid ts0) i
-                                    then Flag.fail
-                                    else Flag.emp));;; trigger Yield;;; Ret ())).
+  (* Let src_code_ind tid: itree ((eventE +' cE) +' sE (Mod.state AbsLockW.mod)) () := *)
+  (*                        (trigger Yield;;; *)
+  (*                         ` x : () + () <- *)
+  (*                         (` x_0 : bool * NatMap.t () <- trigger (Get (bool * NatMap.t ()));; *)
+  (*                          (let (own0, _) := x_0 in *)
+  (*                           if Bool.eqb own0 true then Ret (inl ()) else Ret (inr ())));; *)
+  (*                         match x with *)
+  (*                         | inl l0 => *)
+  (*                             tau;; ITree.iter *)
+  (*                                     (λ _ : (), *)
+  (*                                        trigger Yield;;; *)
+  (*                                        ` x_0 : bool * NatMap.t () <- *)
+  (*                                        trigger (Get (bool * NatMap.t ()));; *)
+  (*                                        (let (own0, _) := x_0 in *)
+  (*                                         if Bool.eqb own0 true *)
+  (*                                         then Ret (inl ()) *)
+  (*                                         else Ret (inr ()))) l0 *)
+  (*                         | inr r0 => Ret r0 *)
+  (*                         end;;; *)
+  (*                         ` x_0 : bool * NatMap.t () <- trigger (Get (bool * NatMap.t ()));; *)
+  (*                         (let (_, ts0) := x_0 in *)
+  (*                          trigger (Put (true, NatMap.remove (elt:=()) tid ts0));;; *)
+  (*                          trigger *)
+  (*                            (Fair *)
+  (*                               (λ i : nat, *)
+  (*                                  if tid_dec i tid *)
+  (*                                  then Flag.success *)
+  (*                                  else *)
+  (*                                   if NatMapP.F.In_dec (NatMap.remove (elt:=()) tid ts0) i *)
+  (*                                   then Flag.fail *)
+  (*                                   else Flag.emp));;; trigger Yield;;; Ret ())). *)
 
-  Let tgt_code_ind mytk now_old :=
-                         (` r : Any.t <-
-                          OMod.embed_itree TicketLock.omod (WMem.mod TicketLock.gvs)
-                            (Mod.wrap_fun WMem.compare_fun
-                               (Any.upcast (WMem.val_nat now_old, WMem.val_nat mytk)));;
-                          ` x : bool <- (tau;; unwrap (Any.downcast r));;
-                          OMod.close_itree TicketLock.omod (WMem.mod TicketLock.gvs)
-                            (if x
-                             then Ret ()
-                             else tau;; TicketLock.lock_loop (WMem.val_nat mytk));;;
-                          OMod.close_itree TicketLock.omod (WMem.mod TicketLock.gvs)
-                            (trigger Yield)).
+  (* Let tgt_code_ind mytk now_old := *)
+  (*                        (` r : Any.t <- *)
+  (*                         OMod.embed_itree TicketLock.omod (WMem.mod TicketLock.gvs) *)
+  (*                           (Mod.wrap_fun WMem.compare_fun *)
+  (*                              (Any.upcast (WMem.val_nat now_old, WMem.val_nat mytk)));; *)
+  (*                         ` x : bool <- (tau;; unwrap (Any.downcast r));; *)
+  (*                         OMod.close_itree TicketLock.omod (WMem.mod TicketLock.gvs) *)
+  (*                           (if x *)
+  (*                            then Ret () *)
+  (*                            else tau;; TicketLock.lock_loop (WMem.val_nat mytk));;; *)
+  (*                         OMod.close_itree TicketLock.omod (WMem.mod TicketLock.gvs) *)
+  (*                           (trigger Yield)). *)
 
-  Lemma lock_yourturn_ind0
-        (g0 g1 : ∀ R_src R_tgt : Type,
-            (R_src → R_tgt → iProp)
-            → bool
-            → bool
-            → itree ((eventE +' cE) +' sE (Mod.state AbsLockW.mod)) R_src
-            → itree ((eventE +' cE) +' sE (OMod.closed_state TicketLock.omod (WMem.mod TicketLock.gvs))) R_tgt → iProp)
-        (tid : nat)
-        (mytk : TicketLockW.tk)
-  (now : nat)
-  (LT : now < mytk)
-  (IH : ∀ y : nat,
-         y < mytk - now
-         → ∀ now_old : nat,
-             mytk ≠ now_old
-             → ∀ (mem : WMem.t) (own : bool) (l : list nat) (tks : NatMap.t nat)
-                 (now next myt : nat),
-                 now < mytk
-                 → y = mytk - now
-                   → (□ ((∀ a : TicketLockW.tk,
-                            (OwnM (Auth.white (NatMapRA.singleton tid a: NatMapRA.t nat)) **
-                             maps_to tid (Auth.white (Excl.just 2: Excl.t nat))) -*
-                            g1 ()%type ()%type
-                              (λ r_src r_tgt : (),
-                                 (own_thread tid ** ObligationRA.duty (inl tid) []) **
-                                 ⌜r_src = r_tgt⌝) false false
-                              (src_code_coind tid)
-                              (tgt_code_coind a)
-                         ) ∧ monoWhite tk_mono Nat.le_preorder now) **
-                      (maps_to tid (Auth.white (Excl.just 2: Excl.t nat)) **
-                       (OwnM (Auth.white (NatMapRA.singleton tid mytk: NatMapRA.t nat)) **
-                        (ticket_lock_inv_tks tks **
-                         (ticket_lock_inv_state mem own tks **
-                          ((⌜own = true⌝ ** ticket_lock_inv_locked l tks now next myt)
-                           ∨ (⌜own = false⌝ **
-                              ticket_lock_inv_unlocking l tks now next myt
-                              ∨ ticket_lock_inv_unlocked0 l tks now next myt
-                                ∨ ticket_lock_inv_unlocked1 l tks now next myt) **
-                           ((ticket_lock_inv -*
-                             MUpd (nth_default True%I I)
-                               (fairI
-                                  (ident_tgt:=OMod.closed_ident TicketLock.omod
-                                                (WMem.mod TicketLock.gvs))) [] [0] True) **
-                            ticket_lock_inv_mem mem now next myt)))))))
-                     ⊢ stsim I tid [] g0 g1
-                         (λ r_src r_tgt : (),
-                            (own_thread tid ** ObligationRA.duty (inl tid) []) ** ⌜r_src = r_tgt⌝)
-                         false true
-                         (src_code_ind tid)
-                         (tgt_code_ind mytk now_old)
-  )
-  (now_old : nat)
-  (NEQ : mytk ≠ now_old)
-  (mem : WMem.t)
-  (l : list nat)
-  (tks : NatMap.t nat)
-  (next myt : nat)
-    :
-  (□ ((∀ a : TicketLockW.tk,
-        (OwnM (Auth.white (NatMapRA.singleton tid a: NatMapRA.t nat)) ** maps_to tid (Auth.white (Excl.just 2: Excl.t nat))) -*
-        g1 ()%type ()%type
-          (λ r_src r_tgt : (),
-             (own_thread tid ** ObligationRA.duty (inl tid) []) ** ⌜r_src = r_tgt⌝) false false
-          (src_code_coind tid)
-          (tgt_code_coind a))
-          ∧
-  (monoWhite tk_mono Nat.le_preorder now)
-     ) **
-   (maps_to tid (Auth.white (Excl.just 2: Excl.t nat)) **
-    (OwnM (Auth.white (NatMapRA.singleton tid mytk: NatMapRA.t nat)) **
-     (ticket_lock_inv_tks tks **
-      (ticket_lock_inv_mem mem now next myt **
-       (ticket_lock_inv_state mem false tks **
-        (ticket_lock_inv_unlocking l tks now next myt **
-         (ticket_lock_inv -*
-          MUpd (nth_default True%I I)
-            (fairI (ident_tgt:=OMod.closed_ident TicketLock.omod (WMem.mod TicketLock.gvs))) []
-            [0] True)))))))
-  )
-  ⊢ (stsim I tid [] g0 g1
-      (λ r_src r_tgt : (), (own_thread tid ** ObligationRA.duty (inl tid) []) ** ⌜r_src = r_tgt⌝)
-      false true
-      (trigger Yield;;;
-       ` x : () + () <-
-       (` x_0 : bool * NatMap.t () <- trigger (Get (bool * NatMap.t ()));;
-        (let (own0, _) := x_0 in if Bool.eqb own0 true then Ret (inl ()) else Ret (inr ())));;
-       match x with
-       | inl l0 =>
-           tau;; ITree.iter
-                   (λ _ : (),
-                      trigger Yield;;;
-                      ` x_0 : bool * NatMap.t () <- trigger (Get (bool * NatMap.t ()));;
-                      (let (own0, _) := x_0 in
-                       if Bool.eqb own0 true then Ret (inl ()) else Ret (inr ()))) l0
-       | inr r0 => Ret r0
-       end;;;
-       ` x_0 : bool * NatMap.t () <- trigger (Get (bool * NatMap.t ()));;
-       (let (_, ts0) := x_0 in
-        trigger (Put (true, NatMap.remove (elt:=()) tid ts0));;;
-        trigger
-          (Fair
-             (λ i : nat,
-                if tid_dec i tid
-                then Flag.success
-                else
-                 if NatMapP.F.In_dec (NatMap.remove (elt:=()) tid ts0) i
-                 then Flag.fail
-                 else Flag.emp));;; trigger Yield;;; Ret ()))
-      (` r : Any.t <-
-       OMod.embed_itree TicketLock.omod (WMem.mod TicketLock.gvs)
-         (Mod.wrap_fun WMem.compare_fun (Any.upcast (WMem.val_nat now_old, WMem.val_nat mytk)));;
-       ` x : bool <- (tau;; unwrap (Any.downcast r));;
-       OMod.close_itree TicketLock.omod (WMem.mod TicketLock.gvs)
-         (if x then Ret () else tau;; TicketLock.lock_loop (WMem.val_nat mytk));;;
-       OMod.close_itree TicketLock.omod (WMem.mod TicketLock.gvs) (trigger Yield))).
-  Proof.
-    iIntros "[#[CIH MONOTK] [MYN [MYTK [TKS [MEM [ST [I K]]]]]]]".
-    iPoseProof (mytk_find_some with "[MYTK TKS]") as "%FIND". iFrame.
-    iPoseProof (unlocking_mono with "I") as "[%TKQ #[% [% [MONOW OBLB]]]]".
-    clear FIND TKQ.
-    iStopProof. move o before IH. revert_until o. pattern o. revert o.
-    apply (well_founded_induction Ord.lt_well_founded).
-    intros o IHo. intros.
-    iIntros "[#[CIH [MONOTK [MONOW BLK]]] [MYN [MYTK [TKS [MEM [ST [I K]]]]]]]".
+  (* Lemma lock_yourturn_ind0 *)
+  (*       (g0 g1 : ∀ R_src R_tgt : Type, *)
+  (*           (R_src → R_tgt → iProp) *)
+  (*           → bool *)
+  (*           → bool *)
+  (*           → itree ((eventE +' cE) +' sE (Mod.state AbsLockW.mod)) R_src *)
+  (*           → itree ((eventE +' cE) +' sE (OMod.closed_state TicketLock.omod (WMem.mod TicketLock.gvs))) R_tgt → iProp) *)
+  (*       (tid : nat) *)
+  (*       (mytk : TicketLockW.tk) *)
+  (* (now : nat) *)
+  (* (LT : now < mytk) *)
+  (* (IH : ∀ y : nat, *)
+  (*        y < mytk - now *)
+  (*        → ∀ now_old : nat, *)
+  (*            mytk ≠ now_old *)
+  (*            → ∀ (mem : WMem.t) (own : bool) (l : list nat) (tks : NatMap.t nat) *)
+  (*                (now next myt : nat), *)
+  (*                now < mytk *)
+  (*                → y = mytk - now *)
+  (*                  → (□ ((∀ a : TicketLockW.tk, *)
+  (*                           (OwnM (Auth.white (NatMapRA.singleton tid a: NatMapRA.t nat)) ** *)
+  (*                            maps_to tid (Auth.white (Excl.just 2: Excl.t nat))) -* *)
+  (*                           g1 ()%type ()%type *)
+  (*                             (λ r_src r_tgt : (), *)
+  (*                                (own_thread tid ** ObligationRA.duty (inl tid) []) ** *)
+  (*                                ⌜r_src = r_tgt⌝) false false *)
+  (*                             (src_code_coind tid) *)
+  (*                             (tgt_code_coind a) *)
+  (*                        ) ∧ monoWhite tk_mono Nat.le_preorder now) ** *)
+  (*                     (maps_to tid (Auth.white (Excl.just 2: Excl.t nat)) ** *)
+  (*                      (OwnM (Auth.white (NatMapRA.singleton tid mytk: NatMapRA.t nat)) ** *)
+  (*                       (ticket_lock_inv_tks tks ** *)
+  (*                        (ticket_lock_inv_state mem own tks ** *)
+  (*                         ((⌜own = true⌝ ** ticket_lock_inv_locked l tks now next myt) *)
+  (*                          ∨ (⌜own = false⌝ ** *)
+  (*                             ticket_lock_inv_unlocking l tks now next myt *)
+  (*                             ∨ ticket_lock_inv_unlocked0 l tks now next myt *)
+  (*                               ∨ ticket_lock_inv_unlocked1 l tks now next myt) ** *)
+  (*                          ((ticket_lock_inv -* *)
+  (*                            MUpd (nth_default True%I I) *)
+  (*                              (fairI *)
+  (*                                 (ident_tgt:=OMod.closed_ident TicketLock.omod *)
+  (*                                               (WMem.mod TicketLock.gvs))) [] [0] True) ** *)
+  (*                           ticket_lock_inv_mem mem now next myt))))))) *)
+  (*                    ⊢ stsim I tid [] g0 g1 *)
+  (*                        (λ r_src r_tgt : (), *)
+  (*                           (own_thread tid ** ObligationRA.duty (inl tid) []) ** ⌜r_src = r_tgt⌝) *)
+  (*                        false true *)
+  (*                        (src_code_ind tid) *)
+  (*                        (tgt_code_ind mytk now_old) *)
+  (* ) *)
+  (* (now_old : nat) *)
+  (* (NEQ : mytk ≠ now_old) *)
+  (* (mem : WMem.t) *)
+  (* (l : list nat) *)
+  (* (tks : NatMap.t nat) *)
+  (* (next myt : nat) *)
+  (*   : *)
+  (* (□ ((∀ a : TicketLockW.tk, *)
+  (*       (OwnM (Auth.white (NatMapRA.singleton tid a: NatMapRA.t nat)) ** maps_to tid (Auth.white (Excl.just 2: Excl.t nat))) -* *)
+  (*       g1 ()%type ()%type *)
+  (*         (λ r_src r_tgt : (), *)
+  (*            (own_thread tid ** ObligationRA.duty (inl tid) []) ** ⌜r_src = r_tgt⌝) false false *)
+  (*         (src_code_coind tid) *)
+  (*         (tgt_code_coind a)) *)
+  (*         ∧ *)
+  (* (monoWhite tk_mono Nat.le_preorder now) *)
+  (*    ) ** *)
+  (*  (maps_to tid (Auth.white (Excl.just 2: Excl.t nat)) ** *)
+  (*   (OwnM (Auth.white (NatMapRA.singleton tid mytk: NatMapRA.t nat)) ** *)
+  (*    (ticket_lock_inv_tks tks ** *)
+  (*     (ticket_lock_inv_mem mem now next myt ** *)
+  (*      (ticket_lock_inv_state mem false tks ** *)
+  (*       (ticket_lock_inv_unlocking l tks now next myt ** *)
+  (*        (ticket_lock_inv -* *)
+  (*         MUpd (nth_default True%I I) *)
+  (*           (fairI (ident_tgt:=OMod.closed_ident TicketLock.omod (WMem.mod TicketLock.gvs))) [] *)
+  (*           [0] True))))))) *)
+  (* ) *)
+  (* ⊢ (stsim I tid [] g0 g1 *)
+  (*     (λ r_src r_tgt : (), (own_thread tid ** ObligationRA.duty (inl tid) []) ** ⌜r_src = r_tgt⌝) *)
+  (*     false true *)
+  (*     (trigger Yield;;; *)
+  (*      ` x : () + () <- *)
+  (*      (` x_0 : bool * NatMap.t () <- trigger (Get (bool * NatMap.t ()));; *)
+  (*       (let (own0, _) := x_0 in if Bool.eqb own0 true then Ret (inl ()) else Ret (inr ())));; *)
+  (*      match x with *)
+  (*      | inl l0 => *)
+  (*          tau;; ITree.iter *)
+  (*                  (λ _ : (), *)
+  (*                     trigger Yield;;; *)
+  (*                     ` x_0 : bool * NatMap.t () <- trigger (Get (bool * NatMap.t ()));; *)
+  (*                     (let (own0, _) := x_0 in *)
+  (*                      if Bool.eqb own0 true then Ret (inl ()) else Ret (inr ()))) l0 *)
+  (*      | inr r0 => Ret r0 *)
+  (*      end;;; *)
+  (*      ` x_0 : bool * NatMap.t () <- trigger (Get (bool * NatMap.t ()));; *)
+  (*      (let (_, ts0) := x_0 in *)
+  (*       trigger (Put (true, NatMap.remove (elt:=()) tid ts0));;; *)
+  (*       trigger *)
+  (*         (Fair *)
+  (*            (λ i : nat, *)
+  (*               if tid_dec i tid *)
+  (*               then Flag.success *)
+  (*               else *)
+  (*                if NatMapP.F.In_dec (NatMap.remove (elt:=()) tid ts0) i *)
+  (*                then Flag.fail *)
+  (*                else Flag.emp));;; trigger Yield;;; Ret ())) *)
+  (*     (` r : Any.t <- *)
+  (*      OMod.embed_itree TicketLock.omod (WMem.mod TicketLock.gvs) *)
+  (*        (Mod.wrap_fun WMem.compare_fun (Any.upcast (WMem.val_nat now_old, WMem.val_nat mytk)));; *)
+  (*      ` x : bool <- (tau;; unwrap (Any.downcast r));; *)
+  (*      OMod.close_itree TicketLock.omod (WMem.mod TicketLock.gvs) *)
+  (*        (if x then Ret () else tau;; TicketLock.lock_loop (WMem.val_nat mytk));;; *)
+  (*      OMod.close_itree TicketLock.omod (WMem.mod TicketLock.gvs) (trigger Yield))). *)
+  (* Proof. *)
+  (*   iIntros "[#[CIH MONOTK] [MYN [MYTK [TKS [MEM [ST [I K]]]]]]]". *)
+  (*   iPoseProof (mytk_find_some with "[MYTK TKS]") as "%FIND". iFrame. *)
+  (*   iPoseProof (unlocking_mono with "I") as "[%TKQ #[% [% [MONOW OBLB]]]]". *)
+  (*   clear FIND TKQ. *)
+  (*   iStopProof. move o before IH. revert_until o. pattern o. revert o. *)
+  (*   apply (well_founded_induction Ord.lt_well_founded). *)
+  (*   intros o IHo. intros. *)
+  (*   iIntros "[#[CIH [MONOTK [MONOW BLK]]] [MYN [MYTK [TKS [MEM [ST [I K]]]]]]]". *)
 
-    unfold Mod.wrap_fun, WMem.compare_fun. rred.
-    iDestruct "MEM" as "[MEM0 [MEM1 [MEM2 MEM3]]]". iDestruct "ST" as "[ST0 ST1]".
-    iApply stsim_getR. iSplit. eauto. rred.
-    iApply stsim_tauR. rred. iApply stsim_tauR. rred.
-    destruct (Nat.eq_dec now_old mytk).
-    { exfalso. clarify. }
-    rred. iApply stsim_tauR.
-    rewrite TicketLock.lock_loop_red. rred. rewrite close_itree_call. rred.
-    iAssert (ticket_lock_inv_mem mem now next myt)%I with "[MEM0 MEM1 MEM2 MEM3]" as "MEM". iFrame.
-    iAssert (ticket_lock_inv_state mem false tks)%I with "[ST0 ST1]" as "ST". iFrame.
-    iMod ("K" with "[TKS MEM ST I]") as "_".
-    { do 7 iExists _. iSplitL "TKS". iFrame. iSplitL "MEM". iFrame. iSplitL "ST". iFrame.
-      iRight. iSplit. auto. iLeft. iFrame.
-    }
-    clear mem l tks next myt now_old NEQ n.
-    rename now into now_past, LT into LTPAST, k into k_past, o into o_past.
+  (*   unfold Mod.wrap_fun, WMem.compare_fun. rred. *)
+  (*   iDestruct "MEM" as "[MEM0 [MEM1 [MEM2 MEM3]]]". iDestruct "ST" as "[ST0 ST1]". *)
+  (*   iApply stsim_getR. iSplit. eauto. rred. *)
+  (*   iApply stsim_tauR. rred. iApply stsim_tauR. rred. *)
+  (*   destruct (Nat.eq_dec now_old mytk). *)
+  (*   { exfalso. clarify. } *)
+  (*   rred. iApply stsim_tauR. *)
+  (*   rewrite TicketLock.lock_loop_red. rred. rewrite close_itree_call. rred. *)
+  (*   iAssert (ticket_lock_inv_mem mem now next myt)%I with "[MEM0 MEM1 MEM2 MEM3]" as "MEM". iFrame. *)
+  (*   iAssert (ticket_lock_inv_state mem false tks)%I with "[ST0 ST1]" as "ST". iFrame. *)
+  (*   iMod ("K" with "[TKS MEM ST I]") as "_". *)
+  (*   { do 7 iExists _. iSplitL "TKS". iFrame. iSplitL "MEM". iFrame. iSplitL "ST". iFrame. *)
+  (*     iRight. iSplit. auto. iLeft. iFrame. *)
+  (*   } *)
+  (*   clear mem l tks next myt now_old NEQ n. *)
+  (*   rename now into now_past, LT into LTPAST, k into k_past, o into o_past. *)
 
-    iopen 0 "I" "K". do 7 iDestruct "I" as "[% I]". iDestruct "I" as "[TKS [MEM [ST CASES]]]".
-    destruct (Nat.eq_dec mytk now); subst.
-    { iClear "CIH".
-      iApply lock_myturn1.
-      iSplitL "MYTK". iFrame. iSplitL "MYN". iFrame. iSplitL "TKS". iFrame.
-      iSplitL "MEM". iFrame. iSplitL "ST". iFrame. iSplitL "CASES". iFrame.
-      iFrame.
-    }
+  (*   iopen 0 "I" "K". do 7 iDestruct "I" as "[% I]". iDestruct "I" as "[TKS [MEM [ST CASES]]]". *)
+  (*   destruct (Nat.eq_dec mytk now); subst. *)
+  (*   { iClear "CIH". *)
+  (*     iApply lock_myturn1. *)
+  (*     iSplitL "MYTK". iFrame. iSplitL "MYN". iFrame. iSplitL "TKS". iFrame. *)
+  (*     iSplitL "MEM". iFrame. iSplitL "ST". iFrame. iSplitL "CASES". iFrame. *)
+  (*     iFrame. *)
+  (*   } *)
 
-    rename n into NEQ.
-    iApply lock_yourturn_yieldR. eapply NEQ.
-    iSplitL "MYTK TKS MEM ST CASES K".
-    iSplitL "MYTK". iFrame. iSplitL "TKS". iFrame. iSplitL "MEM". iFrame.
-    iSplitL "ST". iFrame. iSplitL "CASES". iFrame. iFrame.
-    iIntros "[MYTK _]". rred.
-    clear mem own l tks now next myt NEQ.
-    iopen 0 "I" "K". do 7 iDestruct "I" as "[% I]". iDestruct "I" as "[TKS [MEM [ST CASES]]]".
-    destruct (Nat.eq_dec mytk now); subst.
-    { iClear "CIH".
-      iPoseProof (mytk_find_some with "[MYTK TKS]") as "%FIND". iFrame.
-      iDestruct "CASES" as "[[%CT I] | [%CF [I | [I | I]]]]".
-      { iPoseProof (locked_contra with "I") as "%F". eauto. inv F. }
-      { iPoseProof (unlocking_contra with "I") as "%F". eauto. inv F. }
-      { iPoseProof (unlocked0_contra with "I") as "%F". eauto. inv F. }
-      iPoseProof (unlocked1_mono with "I") as "[%TKQ #[% [% [MYTN _]]]]".
-      iMod ("K" with "[TKS MEM ST I]") as "_".
-      { do 7 iExists _. iSplitL "TKS". iFrame. iSplitL "MEM". iFrame. iSplitL "ST". iFrame.
-        iRight. iSplit. auto. iFrame.
-      }
-      iApply lock_myturn0. 2: iFrame; auto. lia.
-    }
+  (*   rename n into NEQ. *)
+  (*   iApply lock_yourturn_yieldR. eapply NEQ. *)
+  (*   iSplitL "MYTK TKS MEM ST CASES K". *)
+  (*   iSplitL "MYTK". iFrame. iSplitL "TKS". iFrame. iSplitL "MEM". iFrame. *)
+  (*   iSplitL "ST". iFrame. iSplitL "CASES". iFrame. iFrame. *)
+  (*   iIntros "[MYTK _]". rred. *)
+  (*   clear mem own l tks now next myt NEQ. *)
+  (*   iopen 0 "I" "K". do 7 iDestruct "I" as "[% I]". iDestruct "I" as "[TKS [MEM [ST CASES]]]". *)
+  (*   destruct (Nat.eq_dec mytk now); subst. *)
+  (*   { iClear "CIH". *)
+  (*     iPoseProof (mytk_find_some with "[MYTK TKS]") as "%FIND". iFrame. *)
+  (*     iDestruct "CASES" as "[[%CT I] | [%CF [I | [I | I]]]]". *)
+  (*     { iPoseProof (locked_contra with "I") as "%F". eauto. inv F. } *)
+  (*     { iPoseProof (unlocking_contra with "I") as "%F". eauto. inv F. } *)
+  (*     { iPoseProof (unlocked0_contra with "I") as "%F". eauto. inv F. } *)
+  (*     iPoseProof (unlocked1_mono with "I") as "[%TKQ #[% [% [MYTN _]]]]". *)
+  (*     iMod ("K" with "[TKS MEM ST I]") as "_". *)
+  (*     { do 7 iExists _. iSplitL "TKS". iFrame. iSplitL "MEM". iFrame. iSplitL "ST". iFrame. *)
+  (*       iRight. iSplit. auto. iFrame. *)
+  (*     } *)
+  (*     iApply lock_myturn0. 2: iFrame; auto. lia. *)
+  (*   } *)
 
-    rename n into NEQ. unfold Mod.wrap_fun, WMem.load_fun. rred.
-    iDestruct "MEM" as "[MEM0 [MEM1 [MEM2 MEM3]]]". iDestruct "ST" as "[ST0 ST1]".
-    iApply stsim_getR. iSplit. eauto. rred.
-    iApply stsim_tauR. rred.
-    iPoseProof (memory_ra_load with "MEM0 MEM1") as "%LOAD". des. rewrite LOAD. rred.
-    iApply stsim_tauR. rred.
-    rewrite close_itree_call. rred.
-    iApply lock_yourturn_yieldR. eapply NEQ.
-    iSplitL "MYTK TKS MEM0 MEM1 MEM2 MEM3 ST0 ST1 CASES K".
-    iSplitL "MYTK". iFrame. iSplitL "TKS". iFrame. iSplitL "MEM0 MEM1 MEM2 MEM3". iFrame.
-    iSplitL "ST0 ST1". iFrame. iSplitL "CASES". iFrame. iFrame.
-    iIntros "[MYTK RIGHT]". rred.
-    rename now into now_old. clear mem own l tks next myt LOAD LOAD0.
+  (*   rename n into NEQ. unfold Mod.wrap_fun, WMem.load_fun. rred. *)
+  (*   iDestruct "MEM" as "[MEM0 [MEM1 [MEM2 MEM3]]]". iDestruct "ST" as "[ST0 ST1]". *)
+  (*   iApply stsim_getR. iSplit. eauto. rred. *)
+  (*   iApply stsim_tauR. rred. *)
+  (*   iPoseProof (memory_ra_load with "MEM0 MEM1") as "%LOAD". des. rewrite LOAD. rred. *)
+  (*   iApply stsim_tauR. rred. *)
+  (*   rewrite close_itree_call. rred. *)
+  (*   iApply lock_yourturn_yieldR. eapply NEQ. *)
+  (*   iSplitL "MYTK TKS MEM0 MEM1 MEM2 MEM3 ST0 ST1 CASES K". *)
+  (*   iSplitL "MYTK". iFrame. iSplitL "TKS". iFrame. iSplitL "MEM0 MEM1 MEM2 MEM3". iFrame. *)
+  (*   iSplitL "ST0 ST1". iFrame. iSplitL "CASES". iFrame. iFrame. *)
+  (*   iIntros "[MYTK RIGHT]". rred. *)
+  (*   rename now into now_old. clear mem own l tks next myt LOAD LOAD0. *)
 
-    iopen 0 "I" "K". do 7 iDestruct "I" as "[% I]". iDestruct "I" as "[TKS [MEM [ST CASES]]]".
-    destruct (Nat.eq_dec mytk now); subst.
-    { iClear "CIH". iApply lock_myturn2. auto.
-      iSplitL "MYTK". iFrame. iSplitL "MYN". iFrame. iSplitL "TKS". iFrame.
-      iSplitL "MEM". iFrame. iSplitL "ST". iFrame. iSplitL "CASES". iFrame.
-      iFrame.
-    }
+  (*   iopen 0 "I" "K". do 7 iDestruct "I" as "[% I]". iDestruct "I" as "[TKS [MEM [ST CASES]]]". *)
+  (*   destruct (Nat.eq_dec mytk now); subst. *)
+  (*   { iClear "CIH". iApply lock_myturn2. auto. *)
+  (*     iSplitL "MYTK". iFrame. iSplitL "MYN". iFrame. iSplitL "TKS". iFrame. *)
+  (*     iSplitL "MEM". iFrame. iSplitL "ST". iFrame. iSplitL "CASES". iFrame. *)
+  (*     iFrame. *)
+  (*   } *)
 
-    iPoseProof (mytk_find_some with "[MYTK TKS]") as "%FIND". iFrame.
-    rename n into NEQ2. iPoseProof (yourturn_range with "CASES") as "%LT". eapply FIND. auto.
-    clear NEQ2. iDestruct "CASES" as "[[%CT I] | [%CF [I | [I | I]]]]".
-    { subst own. iApply lock_yourturn_coind. auto. iSplit. iApply "CIH".
-      iSplitL "MYN". iFrame. iSplitL "MYTK". iFrame. iSplitL "TKS". iFrame.
-      iSplitL "MEM". iFrame. iSplitL "ST". iFrame. iSplitL "I". iFrame. iFrame.
-    }
+  (*   iPoseProof (mytk_find_some with "[MYTK TKS]") as "%FIND". iFrame. *)
+  (*   rename n into NEQ2. iPoseProof (yourturn_range with "CASES") as "%LT". eapply FIND. auto. *)
+  (*   clear NEQ2. iDestruct "CASES" as "[[%CT I] | [%CF [I | [I | I]]]]". *)
+  (*   { subst own. iApply lock_yourturn_coind. auto. iSplit. iApply "CIH". *)
+  (*     iSplitL "MYN". iFrame. iSplitL "MYTK". iFrame. iSplitL "TKS". iFrame. *)
+  (*     iSplitL "MEM". iFrame. iSplitL "ST". iFrame. iSplitL "I". iFrame. iFrame. *)
+  (*   } *)
 
-    { iPoseProof (ticket_lock_inv_mem_mono with "MEM") as "#MONOTK2".
-      iDestruct "I" as "[I0 [%I1 [I2 [I3 I4]]]]".
-      do 2 iDestruct "I4" as "[% I4]". iDestruct "I4" as "[I4 [I5 [I6 I7]]]".
-      iPoseProof (black_white_compare with "MONOW I4") as "%LE".
-      inv LE.
-      { remember (mytk - now) as ind. specialize (IH ind).
-        iApply IH.
-        { subst ind. lia. }
-        { auto. }
-        { eapply LT. }
-        { eapply Heqind. }
-        iSplit.
-        { iClear "MYN MYTK RIGHT TKS MEM ST I0 I2 I3 I4 I5 I6 I7 K".
-          iModIntro. iSplit. iApply "CIH". auto.
-        }
-        iSplitL "MYN". iFrame. iSplitL "MYTK". iFrame. iSplitL "TKS". iFrame.
-        iSplitL "ST". iFrame. iSplitR "K MEM". 2: iFrame.
-        iRight. iSplit. auto. iLeft. iFrame. iSplit. auto. iExists _, _. iFrame.
-      }
-      { inv ORD. hexploit H0. lia. i. clear H H0. subst k.
-        iClear "MONOTK2".
-        iPoseProof (ObligationRA.duty_correl_thread with "I7") as "#COR".
-        { ss. left; eauto. }
-        iPoseProof (ObligationRA.correl_thread_correlate with "COR RIGHT") as ">[DROP | FF]".
-        2:{ iPoseProof (ObligationRA.pending_not_shot with "I6 FF") as "%FF". inv FF. }
-        iPoseProof (ObligationRA.black_white_decr with "BLK DROP") as ">[%o_now [#OBLK2 %DROP]]".
-        iClear "BLK".
-        specialize (IHo o_now).
-        iApply IHo.
-        { rewrite Hessenberg.add_S_r in DROP. rewrite Hessenberg.add_O_r in DROP.
-          eapply Ord.lt_le_lt. 2: eapply DROP. apply Ord.S_lt.
-        }
-        { auto. }
-        iSplit.
-        { iClear "MYN MYTK TKS MEM ST I0 I2 I3 I4 I5 I6 I7 K".
-          iModIntro. iSplit. iApply "CIH". iSplit; auto.
-        }
-        iSplitL "MYN". iFrame. iSplitL "MYTK". iFrame. iSplitL "TKS". iFrame.
-        iSplitL "MEM". iFrame. iSplitL "ST". iFrame. iSplitR "K". 2: iFrame.
-        iFrame. iSplit. auto. iExists _, _. iFrame.
-      }
-    }
-    { iPoseProof (unlocked0_contra with "I") as "%FF". eauto. inv FF. }
+  (*   { iPoseProof (ticket_lock_inv_mem_mono with "MEM") as "#MONOTK2". *)
+  (*     iDestruct "I" as "[I0 [%I1 [I2 [I3 I4]]]]". *)
+  (*     do 2 iDestruct "I4" as "[% I4]". iDestruct "I4" as "[I4 [I5 [I6 I7]]]". *)
+  (*     iPoseProof (black_white_compare with "MONOW I4") as "%LE". *)
+  (*     inv LE. *)
+  (*     { remember (mytk - now) as ind. specialize (IH ind). *)
+  (*       iApply IH. *)
+  (*       { subst ind. lia. } *)
+  (*       { auto. } *)
+  (*       { eapply LT. } *)
+  (*       { eapply Heqind. } *)
+  (*       iSplit. *)
+  (*       { iClear "MYN MYTK RIGHT TKS MEM ST I0 I2 I3 I4 I5 I6 I7 K". *)
+  (*         iModIntro. iSplit. iApply "CIH". auto. *)
+  (*       } *)
+  (*       iSplitL "MYN". iFrame. iSplitL "MYTK". iFrame. iSplitL "TKS". iFrame. *)
+  (*       iSplitL "ST". iFrame. iSplitR "K MEM". 2: iFrame. *)
+  (*       iRight. iSplit. auto. iLeft. iFrame. iSplit. auto. iExists _, _. iFrame. *)
+  (*     } *)
+  (*     { inv ORD. hexploit H0. lia. i. clear H H0. subst k. *)
+  (*       iClear "MONOTK2". *)
+  (*       iPoseProof (ObligationRA.duty_correl_thread with "I7") as "#COR". *)
+  (*       { ss. left; eauto. } *)
+  (*       iPoseProof (ObligationRA.correl_thread_correlate with "COR RIGHT") as ">[DROP | FF]". *)
+  (*       2:{ iPoseProof (ObligationRA.pending_not_shot with "I6 FF") as "%FF". inv FF. } *)
+  (*       iPoseProof (ObligationRA.black_white_decr with "BLK DROP") as ">[%o_now [#OBLK2 %DROP]]". *)
+  (*       iClear "BLK". *)
+  (*       specialize (IHo o_now). *)
+  (*       iApply IHo. *)
+  (*       { rewrite Hessenberg.add_S_r in DROP. rewrite Hessenberg.add_O_r in DROP. *)
+  (*         eapply Ord.lt_le_lt. 2: eapply DROP. apply Ord.S_lt. *)
+  (*       } *)
+  (*       { auto. } *)
+  (*       iSplit. *)
+  (*       { iClear "MYN MYTK TKS MEM ST I0 I2 I3 I4 I5 I6 I7 K". *)
+  (*         iModIntro. iSplit. iApply "CIH". iSplit; auto. *)
+  (*       } *)
+  (*       iSplitL "MYN". iFrame. iSplitL "MYTK". iFrame. iSplitL "TKS". iFrame. *)
+  (*       iSplitL "MEM". iFrame. iSplitL "ST". iFrame. iSplitR "K". 2: iFrame. *)
+  (*       iFrame. iSplit. auto. iExists _, _. iFrame. *)
+  (*     } *)
+  (*   } *)
+  (*   { iPoseProof (unlocked0_contra with "I") as "%FF". eauto. inv FF. } *)
 
-    { iPoseProof (ticket_lock_inv_mem_mono with "MEM") as "#MONOTK2".
-      do 2 iDestruct "I" as "[% I]". iDestruct "I" as "[I0 [I1 [%I2 [I3 [I4 I5]]]]]".
-      do 3 iDestruct "I5" as "[% I5]". iDestruct "I5" as "[I5 [I6 [I7 [I8 [I9 I10]]]]]".
-      iPoseProof (black_white_compare with "MONOW I5") as "%LE".
-      inv LE.
-      { remember (mytk - now) as ind. specialize (IH ind).
-        iApply IH.
-        { subst ind. lia. }
-        { auto. }
-        { eapply LT. }
-        { eapply Heqind. }
-        iSplit.
-        { iClear "MYN MYTK RIGHT TKS MEM ST I0 I1 I3 I4 I5 I6 I7 I8 I9 I10 K".
-          iModIntro. iSplit. iApply "CIH". auto.
-        }
-        iSplitL "MYN". iFrame. iSplitL "MYTK". iFrame. iSplitL "TKS". iFrame.
-        iSplitL "ST". iFrame. iSplitR "K MEM". 2: iFrame.
-        iRight. iSplit. auto. iRight. iRight. iFrame.
-        iExists yourt, waits. iSplit. auto. iSplit. auto. iFrame.
-        iExists k, o, u. iFrame.
-      }
-      { exfalso. inv ORD. lia. }
-    }
-  Qed.
+  (*   { iPoseProof (ticket_lock_inv_mem_mono with "MEM") as "#MONOTK2". *)
+  (*     do 2 iDestruct "I" as "[% I]". iDestruct "I" as "[I0 [I1 [%I2 [I3 [I4 I5]]]]]". *)
+  (*     do 3 iDestruct "I5" as "[% I5]". iDestruct "I5" as "[I5 [I6 [I7 [I8 [I9 I10]]]]]". *)
+  (*     iPoseProof (black_white_compare with "MONOW I5") as "%LE". *)
+  (*     inv LE. *)
+  (*     { remember (mytk - now) as ind. specialize (IH ind). *)
+  (*       iApply IH. *)
+  (*       { subst ind. lia. } *)
+  (*       { auto. } *)
+  (*       { eapply LT. } *)
+  (*       { eapply Heqind. } *)
+  (*       iSplit. *)
+  (*       { iClear "MYN MYTK RIGHT TKS MEM ST I0 I1 I3 I4 I5 I6 I7 I8 I9 I10 K". *)
+  (*         iModIntro. iSplit. iApply "CIH". auto. *)
+  (*       } *)
+  (*       iSplitL "MYN". iFrame. iSplitL "MYTK". iFrame. iSplitL "TKS". iFrame. *)
+  (*       iSplitL "ST". iFrame. iSplitR "K MEM". 2: iFrame. *)
+  (*       iRight. iSplit. auto. iRight. iRight. iFrame. *)
+  (*       iExists yourt, waits. iSplit. auto. iSplit. auto. iFrame. *)
+  (*       iExists k, o, u. iFrame. *)
+  (*     } *)
+  (*     { exfalso. inv ORD. lia. } *)
+  (*   } *)
+  (* Qed. *)
 
-  Lemma lock_yourturn_ind1
-        (g0 g1 : ∀ R_src R_tgt : Type,
-            (R_src → R_tgt → iProp)
-            → bool
-            → bool
-            → itree ((eventE +' cE) +' sE (Mod.state AbsLockW.mod)) R_src
-            → itree ((eventE +' cE) +' sE (OMod.closed_state TicketLock.omod (WMem.mod TicketLock.gvs))) R_tgt → iProp)
-        (tid : nat)
-        (mytk : TicketLockW.tk)
-  (now : nat)
-  (LT : now < mytk)
-  (IH : ∀ y : nat,
-         y < mytk - now
-         → ∀ now_old : nat,
-             mytk ≠ now_old
-             → ∀ (mem : WMem.t) (own : bool) (l : list nat) (tks : NatMap.t nat)
-                 (now next myt : nat),
-                 now < mytk
-                 → y = mytk - now
-                   → (□ ((∀ a : TicketLockW.tk,
-                            (OwnM (Auth.white (NatMapRA.singleton tid a: NatMapRA.t nat)) **
-                             maps_to tid (Auth.white (Excl.just 2: Excl.t nat))) -*
-                            g1 ()%type ()%type
-                              (λ r_src r_tgt : (),
-                                 (own_thread tid ** ObligationRA.duty (inl tid) []) **
-                                 ⌜r_src = r_tgt⌝) false false
-                              (src_code_coind tid)
-                              (tgt_code_coind a)
-                         ) ∧ monoWhite tk_mono Nat.le_preorder now) **
-                      (maps_to tid (Auth.white (Excl.just 2: Excl.t nat)) **
-                       (OwnM (Auth.white (NatMapRA.singleton tid mytk: NatMapRA.t nat)) **
-                        (ticket_lock_inv_tks tks **
-                         (ticket_lock_inv_state mem own tks **
-                          ((⌜own = true⌝ ** ticket_lock_inv_locked l tks now next myt)
-                           ∨ (⌜own = false⌝ **
-                              ticket_lock_inv_unlocking l tks now next myt
-                              ∨ ticket_lock_inv_unlocked0 l tks now next myt
-                                ∨ ticket_lock_inv_unlocked1 l tks now next myt) **
-                           ((ticket_lock_inv -*
-                             MUpd (nth_default True%I I)
-                               (fairI
-                                  (ident_tgt:=OMod.closed_ident TicketLock.omod
-                                                (WMem.mod TicketLock.gvs))) [] [0] True) **
-                            ticket_lock_inv_mem mem now next myt)))))))
-                     ⊢ stsim I tid [] g0 g1
-                         (λ r_src r_tgt : (),
-                            (own_thread tid ** ObligationRA.duty (inl tid) []) ** ⌜r_src = r_tgt⌝)
-                         false true
-                         (src_code_ind tid)
-                         (tgt_code_ind mytk now_old)
-  )
-  (now_old : nat)
-  (NEQ : mytk ≠ now_old)
-  (mem : WMem.t)
-  (l : list nat)
-  (tks : NatMap.t nat)
-  (next myt : nat)
-    :
-  (□ ((∀ a : TicketLockW.tk,
-        (OwnM (Auth.white (NatMapRA.singleton tid a: NatMapRA.t nat)) ** maps_to tid (Auth.white (Excl.just 2: Excl.t nat))) -*
-        g1 ()%type ()%type
-          (λ r_src r_tgt : (),
-             (own_thread tid ** ObligationRA.duty (inl tid) []) ** ⌜r_src = r_tgt⌝) false false
-          (src_code_coind tid)
-          (tgt_code_coind a))
-          ∧
-  (monoWhite tk_mono Nat.le_preorder now)
-     ) **
-   (maps_to tid (Auth.white (Excl.just 2: Excl.t nat)) **
-    (OwnM (Auth.white (NatMapRA.singleton tid mytk: NatMapRA.t nat)) **
-     (ticket_lock_inv_tks tks **
-      (ticket_lock_inv_mem mem now next myt **
-       (ticket_lock_inv_state mem false tks **
-        (ticket_lock_inv_unlocked1 l tks now next myt **
-         (ticket_lock_inv -*
-          MUpd (nth_default True%I I)
-            (fairI (ident_tgt:=OMod.closed_ident TicketLock.omod (WMem.mod TicketLock.gvs))) []
-            [0] True)))))))
-  )
-  ⊢ (stsim I tid [] g0 g1
-      (λ r_src r_tgt : (), (own_thread tid ** ObligationRA.duty (inl tid) []) ** ⌜r_src = r_tgt⌝)
-      false true
-      (trigger Yield;;;
-       ` x : () + () <-
-       (` x_0 : bool * NatMap.t () <- trigger (Get (bool * NatMap.t ()));;
-        (let (own0, _) := x_0 in if Bool.eqb own0 true then Ret (inl ()) else Ret (inr ())));;
-       match x with
-       | inl l0 =>
-           tau;; ITree.iter
-                   (λ _ : (),
-                      trigger Yield;;;
-                      ` x_0 : bool * NatMap.t () <- trigger (Get (bool * NatMap.t ()));;
-                      (let (own0, _) := x_0 in
-                       if Bool.eqb own0 true then Ret (inl ()) else Ret (inr ()))) l0
-       | inr r0 => Ret r0
-       end;;;
-       ` x_0 : bool * NatMap.t () <- trigger (Get (bool * NatMap.t ()));;
-       (let (_, ts0) := x_0 in
-        trigger (Put (true, NatMap.remove (elt:=()) tid ts0));;;
-        trigger
-          (Fair
-             (λ i : nat,
-                if tid_dec i tid
-                then Flag.success
-                else
-                 if NatMapP.F.In_dec (NatMap.remove (elt:=()) tid ts0) i
-                 then Flag.fail
-                 else Flag.emp));;; trigger Yield;;; Ret ()))
-      (` r : Any.t <-
-       OMod.embed_itree TicketLock.omod (WMem.mod TicketLock.gvs)
-         (Mod.wrap_fun WMem.compare_fun (Any.upcast (WMem.val_nat now_old, WMem.val_nat mytk)));;
-       ` x : bool <- (tau;; unwrap (Any.downcast r));;
-       OMod.close_itree TicketLock.omod (WMem.mod TicketLock.gvs)
-         (if x then Ret () else tau;; TicketLock.lock_loop (WMem.val_nat mytk));;;
-       OMod.close_itree TicketLock.omod (WMem.mod TicketLock.gvs) (trigger Yield))).
-  Proof.
-    iIntros "[#[CIH MONOTK] [MYN [MYTK [TKS [MEM [ST [I K]]]]]]]".
-    iPoseProof (mytk_find_some with "[MYTK TKS]") as "%FIND". iFrame.
-    iPoseProof (unlocked1_mono with "I") as "[%TKQ #[% [% [MONOW OBLB]]]]".
-    clear FIND TKQ.
-    iStopProof. move o before IH. revert_until o. pattern o. revert o.
-    apply (well_founded_induction Ord.lt_well_founded).
-    intros o IHo. intros.
-    iIntros "[#[CIH [MONOTK [MONOW BLK]]] [MYN [MYTK [TKS [MEM [ST [I K]]]]]]]".
+  (* Lemma lock_yourturn_ind1 *)
+  (*       (g0 g1 : ∀ R_src R_tgt : Type, *)
+  (*           (R_src → R_tgt → iProp) *)
+  (*           → bool *)
+  (*           → bool *)
+  (*           → itree ((eventE +' cE) +' sE (Mod.state AbsLockW.mod)) R_src *)
+  (*           → itree ((eventE +' cE) +' sE (OMod.closed_state TicketLock.omod (WMem.mod TicketLock.gvs))) R_tgt → iProp) *)
+  (*       (tid : nat) *)
+  (*       (mytk : TicketLockW.tk) *)
+  (* (now : nat) *)
+  (* (LT : now < mytk) *)
+  (* (IH : ∀ y : nat, *)
+  (*        y < mytk - now *)
+  (*        → ∀ now_old : nat, *)
+  (*            mytk ≠ now_old *)
+  (*            → ∀ (mem : WMem.t) (own : bool) (l : list nat) (tks : NatMap.t nat) *)
+  (*                (now next myt : nat), *)
+  (*                now < mytk *)
+  (*                → y = mytk - now *)
+  (*                  → (□ ((∀ a : TicketLockW.tk, *)
+  (*                           (OwnM (Auth.white (NatMapRA.singleton tid a: NatMapRA.t nat)) ** *)
+  (*                            maps_to tid (Auth.white (Excl.just 2: Excl.t nat))) -* *)
+  (*                           g1 ()%type ()%type *)
+  (*                             (λ r_src r_tgt : (), *)
+  (*                                (own_thread tid ** ObligationRA.duty (inl tid) []) ** *)
+  (*                                ⌜r_src = r_tgt⌝) false false *)
+  (*                             (src_code_coind tid) *)
+  (*                             (tgt_code_coind a) *)
+  (*                        ) ∧ monoWhite tk_mono Nat.le_preorder now) ** *)
+  (*                     (maps_to tid (Auth.white (Excl.just 2: Excl.t nat)) ** *)
+  (*                      (OwnM (Auth.white (NatMapRA.singleton tid mytk: NatMapRA.t nat)) ** *)
+  (*                       (ticket_lock_inv_tks tks ** *)
+  (*                        (ticket_lock_inv_state mem own tks ** *)
+  (*                         ((⌜own = true⌝ ** ticket_lock_inv_locked l tks now next myt) *)
+  (*                          ∨ (⌜own = false⌝ ** *)
+  (*                             ticket_lock_inv_unlocking l tks now next myt *)
+  (*                             ∨ ticket_lock_inv_unlocked0 l tks now next myt *)
+  (*                               ∨ ticket_lock_inv_unlocked1 l tks now next myt) ** *)
+  (*                          ((ticket_lock_inv -* *)
+  (*                            MUpd (nth_default True%I I) *)
+  (*                              (fairI *)
+  (*                                 (ident_tgt:=OMod.closed_ident TicketLock.omod *)
+  (*                                               (WMem.mod TicketLock.gvs))) [] [0] True) ** *)
+  (*                           ticket_lock_inv_mem mem now next myt))))))) *)
+  (*                    ⊢ stsim I tid [] g0 g1 *)
+  (*                        (λ r_src r_tgt : (), *)
+  (*                           (own_thread tid ** ObligationRA.duty (inl tid) []) ** ⌜r_src = r_tgt⌝) *)
+  (*                        false true *)
+  (*                        (src_code_ind tid) *)
+  (*                        (tgt_code_ind mytk now_old) *)
+  (* ) *)
+  (* (now_old : nat) *)
+  (* (NEQ : mytk ≠ now_old) *)
+  (* (mem : WMem.t) *)
+  (* (l : list nat) *)
+  (* (tks : NatMap.t nat) *)
+  (* (next myt : nat) *)
+  (*   : *)
+  (* (□ ((∀ a : TicketLockW.tk, *)
+  (*       (OwnM (Auth.white (NatMapRA.singleton tid a: NatMapRA.t nat)) ** maps_to tid (Auth.white (Excl.just 2: Excl.t nat))) -* *)
+  (*       g1 ()%type ()%type *)
+  (*         (λ r_src r_tgt : (), *)
+  (*            (own_thread tid ** ObligationRA.duty (inl tid) []) ** ⌜r_src = r_tgt⌝) false false *)
+  (*         (src_code_coind tid) *)
+  (*         (tgt_code_coind a)) *)
+  (*         ∧ *)
+  (* (monoWhite tk_mono Nat.le_preorder now) *)
+  (*    ) ** *)
+  (*  (maps_to tid (Auth.white (Excl.just 2: Excl.t nat)) ** *)
+  (*   (OwnM (Auth.white (NatMapRA.singleton tid mytk: NatMapRA.t nat)) ** *)
+  (*    (ticket_lock_inv_tks tks ** *)
+  (*     (ticket_lock_inv_mem mem now next myt ** *)
+  (*      (ticket_lock_inv_state mem false tks ** *)
+  (*       (ticket_lock_inv_unlocked1 l tks now next myt ** *)
+  (*        (ticket_lock_inv -* *)
+  (*         MUpd (nth_default True%I I) *)
+  (*           (fairI (ident_tgt:=OMod.closed_ident TicketLock.omod (WMem.mod TicketLock.gvs))) [] *)
+  (*           [0] True))))))) *)
+  (* ) *)
+  (* ⊢ (stsim I tid [] g0 g1 *)
+  (*     (λ r_src r_tgt : (), (own_thread tid ** ObligationRA.duty (inl tid) []) ** ⌜r_src = r_tgt⌝) *)
+  (*     false true *)
+  (*     (trigger Yield;;; *)
+  (*      ` x : () + () <- *)
+  (*      (` x_0 : bool * NatMap.t () <- trigger (Get (bool * NatMap.t ()));; *)
+  (*       (let (own0, _) := x_0 in if Bool.eqb own0 true then Ret (inl ()) else Ret (inr ())));; *)
+  (*      match x with *)
+  (*      | inl l0 => *)
+  (*          tau;; ITree.iter *)
+  (*                  (λ _ : (), *)
+  (*                     trigger Yield;;; *)
+  (*                     ` x_0 : bool * NatMap.t () <- trigger (Get (bool * NatMap.t ()));; *)
+  (*                     (let (own0, _) := x_0 in *)
+  (*                      if Bool.eqb own0 true then Ret (inl ()) else Ret (inr ()))) l0 *)
+  (*      | inr r0 => Ret r0 *)
+  (*      end;;; *)
+  (*      ` x_0 : bool * NatMap.t () <- trigger (Get (bool * NatMap.t ()));; *)
+  (*      (let (_, ts0) := x_0 in *)
+  (*       trigger (Put (true, NatMap.remove (elt:=()) tid ts0));;; *)
+  (*       trigger *)
+  (*         (Fair *)
+  (*            (λ i : nat, *)
+  (*               if tid_dec i tid *)
+  (*               then Flag.success *)
+  (*               else *)
+  (*                if NatMapP.F.In_dec (NatMap.remove (elt:=()) tid ts0) i *)
+  (*                then Flag.fail *)
+  (*                else Flag.emp));;; trigger Yield;;; Ret ())) *)
+  (*     (` r : Any.t <- *)
+  (*      OMod.embed_itree TicketLock.omod (WMem.mod TicketLock.gvs) *)
+  (*        (Mod.wrap_fun WMem.compare_fun (Any.upcast (WMem.val_nat now_old, WMem.val_nat mytk)));; *)
+  (*      ` x : bool <- (tau;; unwrap (Any.downcast r));; *)
+  (*      OMod.close_itree TicketLock.omod (WMem.mod TicketLock.gvs) *)
+  (*        (if x then Ret () else tau;; TicketLock.lock_loop (WMem.val_nat mytk));;; *)
+  (*      OMod.close_itree TicketLock.omod (WMem.mod TicketLock.gvs) (trigger Yield))). *)
+  (* Proof. *)
+  (*   iIntros "[#[CIH MONOTK] [MYN [MYTK [TKS [MEM [ST [I K]]]]]]]". *)
+  (*   iPoseProof (mytk_find_some with "[MYTK TKS]") as "%FIND". iFrame. *)
+  (*   iPoseProof (unlocked1_mono with "I") as "[%TKQ #[% [% [MONOW OBLB]]]]". *)
+  (*   clear FIND TKQ. *)
+  (*   iStopProof. move o before IH. revert_until o. pattern o. revert o. *)
+  (*   apply (well_founded_induction Ord.lt_well_founded). *)
+  (*   intros o IHo. intros. *)
+  (*   iIntros "[#[CIH [MONOTK [MONOW BLK]]] [MYN [MYTK [TKS [MEM [ST [I K]]]]]]]". *)
 
-    unfold Mod.wrap_fun, WMem.compare_fun. rred.
-    iDestruct "MEM" as "[MEM0 [MEM1 [MEM2 MEM3]]]". iDestruct "ST" as "[ST0 ST1]".
-    iApply stsim_getR. iSplit. eauto. rred.
-    iApply stsim_tauR. rred. iApply stsim_tauR. rred.
-    destruct (Nat.eq_dec now_old mytk).
-    { exfalso. clarify. }
-    rred. iApply stsim_tauR.
-    rewrite TicketLock.lock_loop_red. rred. rewrite close_itree_call. rred.
-    iAssert (ticket_lock_inv_mem mem now next myt)%I with "[MEM0 MEM1 MEM2 MEM3]" as "MEM". iFrame.
-    iAssert (ticket_lock_inv_state mem false tks)%I with "[ST0 ST1]" as "ST". iFrame.
-    iMod ("K" with "[TKS MEM ST I]") as "_".
-    { do 7 iExists _. iSplitL "TKS". iFrame. iSplitL "MEM". iFrame. iSplitL "ST". iFrame.
-      iRight. iSplit. auto. iRight. iRight. iFrame.
-    }
-    clear mem l tks next myt now_old NEQ n.
-    rename now into now_past, LT into LTPAST, k into k_past, o into o_past.
+  (*   unfold Mod.wrap_fun, WMem.compare_fun. rred. *)
+  (*   iDestruct "MEM" as "[MEM0 [MEM1 [MEM2 MEM3]]]". iDestruct "ST" as "[ST0 ST1]". *)
+  (*   iApply stsim_getR. iSplit. eauto. rred. *)
+  (*   iApply stsim_tauR. rred. iApply stsim_tauR. rred. *)
+  (*   destruct (Nat.eq_dec now_old mytk). *)
+  (*   { exfalso. clarify. } *)
+  (*   rred. iApply stsim_tauR. *)
+  (*   rewrite TicketLock.lock_loop_red. rred. rewrite close_itree_call. rred. *)
+  (*   iAssert (ticket_lock_inv_mem mem now next myt)%I with "[MEM0 MEM1 MEM2 MEM3]" as "MEM". iFrame. *)
+  (*   iAssert (ticket_lock_inv_state mem false tks)%I with "[ST0 ST1]" as "ST". iFrame. *)
+  (*   iMod ("K" with "[TKS MEM ST I]") as "_". *)
+  (*   { do 7 iExists _. iSplitL "TKS". iFrame. iSplitL "MEM". iFrame. iSplitL "ST". iFrame. *)
+  (*     iRight. iSplit. auto. iRight. iRight. iFrame. *)
+  (*   } *)
+  (*   clear mem l tks next myt now_old NEQ n. *)
+  (*   rename now into now_past, LT into LTPAST, k into k_past, o into o_past. *)
 
-    iopen 0 "I" "K". do 7 iDestruct "I" as "[% I]". iDestruct "I" as "[TKS [MEM [ST CASES]]]".
-    destruct (Nat.eq_dec mytk now); subst.
-    { iClear "CIH".
-      iApply lock_myturn1.
-      iSplitL "MYTK". iFrame. iSplitL "MYN". iFrame. iSplitL "TKS". iFrame.
-      iSplitL "MEM". iFrame. iSplitL "ST". iFrame. iSplitL "CASES". iFrame.
-      iFrame.
-    }
+  (*   iopen 0 "I" "K". do 7 iDestruct "I" as "[% I]". iDestruct "I" as "[TKS [MEM [ST CASES]]]". *)
+  (*   destruct (Nat.eq_dec mytk now); subst. *)
+  (*   { iClear "CIH". *)
+  (*     iApply lock_myturn1. *)
+  (*     iSplitL "MYTK". iFrame. iSplitL "MYN". iFrame. iSplitL "TKS". iFrame. *)
+  (*     iSplitL "MEM". iFrame. iSplitL "ST". iFrame. iSplitL "CASES". iFrame. *)
+  (*     iFrame. *)
+  (*   } *)
 
-    rename n into NEQ.
-    iApply lock_yourturn_yieldR. eapply NEQ.
-    iSplitL "MYTK TKS MEM ST CASES K".
-    iSplitL "MYTK". iFrame. iSplitL "TKS". iFrame. iSplitL "MEM". iFrame.
-    iSplitL "ST". iFrame. iSplitL "CASES". iFrame. iFrame.
-    iIntros "[MYTK _]". rred.
-    clear mem own l tks now next myt NEQ.
-    iopen 0 "I" "K". do 7 iDestruct "I" as "[% I]". iDestruct "I" as "[TKS [MEM [ST CASES]]]".
-    destruct (Nat.eq_dec mytk now); subst.
-    { iClear "CIH".
-      iPoseProof (mytk_find_some with "[MYTK TKS]") as "%FIND". iFrame.
-      iDestruct "CASES" as "[[%CT I] | [%CF [I | [I | I]]]]".
-      { iPoseProof (locked_contra with "I") as "%F". eauto. inv F. }
-      { iPoseProof (unlocking_contra with "I") as "%F". eauto. inv F. }
-      { iPoseProof (unlocked0_contra with "I") as "%F". eauto. inv F. }
-      iPoseProof (unlocked1_mono with "I") as "[%TKQ #[% [% [MYTN _]]]]".
-      iMod ("K" with "[TKS MEM ST I]") as "_".
-      { do 7 iExists _. iSplitL "TKS". iFrame. iSplitL "MEM". iFrame. iSplitL "ST". iFrame.
-        iRight. iSplit. auto. iFrame.
-      }
-      iApply lock_myturn0. 2: iFrame; auto. lia.
-    }
+  (*   rename n into NEQ. *)
+  (*   iApply lock_yourturn_yieldR. eapply NEQ. *)
+  (*   iSplitL "MYTK TKS MEM ST CASES K". *)
+  (*   iSplitL "MYTK". iFrame. iSplitL "TKS". iFrame. iSplitL "MEM". iFrame. *)
+  (*   iSplitL "ST". iFrame. iSplitL "CASES". iFrame. iFrame. *)
+  (*   iIntros "[MYTK _]". rred. *)
+  (*   clear mem own l tks now next myt NEQ. *)
+  (*   iopen 0 "I" "K". do 7 iDestruct "I" as "[% I]". iDestruct "I" as "[TKS [MEM [ST CASES]]]". *)
+  (*   destruct (Nat.eq_dec mytk now); subst. *)
+  (*   { iClear "CIH". *)
+  (*     iPoseProof (mytk_find_some with "[MYTK TKS]") as "%FIND". iFrame. *)
+  (*     iDestruct "CASES" as "[[%CT I] | [%CF [I | [I | I]]]]". *)
+  (*     { iPoseProof (locked_contra with "I") as "%F". eauto. inv F. } *)
+  (*     { iPoseProof (unlocking_contra with "I") as "%F". eauto. inv F. } *)
+  (*     { iPoseProof (unlocked0_contra with "I") as "%F". eauto. inv F. } *)
+  (*     iPoseProof (unlocked1_mono with "I") as "[%TKQ #[% [% [MYTN _]]]]". *)
+  (*     iMod ("K" with "[TKS MEM ST I]") as "_". *)
+  (*     { do 7 iExists _. iSplitL "TKS". iFrame. iSplitL "MEM". iFrame. iSplitL "ST". iFrame. *)
+  (*       iRight. iSplit. auto. iFrame. *)
+  (*     } *)
+  (*     iApply lock_myturn0. 2: iFrame; auto. lia. *)
+  (*   } *)
 
-    rename n into NEQ. unfold Mod.wrap_fun, WMem.load_fun. rred.
-    iDestruct "MEM" as "[MEM0 [MEM1 [MEM2 MEM3]]]". iDestruct "ST" as "[ST0 ST1]".
-    iApply stsim_getR. iSplit. eauto. rred.
-    iApply stsim_tauR. rred.
-    iPoseProof (memory_ra_load with "MEM0 MEM1") as "%LOAD". des. rewrite LOAD. rred.
-    iApply stsim_tauR. rred.
-    rewrite close_itree_call. rred.
-    iApply lock_yourturn_yieldR. eapply NEQ.
-    iSplitL "MYTK TKS MEM0 MEM1 MEM2 MEM3 ST0 ST1 CASES K".
-    iSplitL "MYTK". iFrame. iSplitL "TKS". iFrame. iSplitL "MEM0 MEM1 MEM2 MEM3". iFrame.
-    iSplitL "ST0 ST1". iFrame. iSplitL "CASES". iFrame. iFrame.
-    iIntros "[MYTK RIGHT]". rred.
-    rename now into now_old. clear mem own l tks next myt LOAD LOAD0.
+  (*   rename n into NEQ. unfold Mod.wrap_fun, WMem.load_fun. rred. *)
+  (*   iDestruct "MEM" as "[MEM0 [MEM1 [MEM2 MEM3]]]". iDestruct "ST" as "[ST0 ST1]". *)
+  (*   iApply stsim_getR. iSplit. eauto. rred. *)
+  (*   iApply stsim_tauR. rred. *)
+  (*   iPoseProof (memory_ra_load with "MEM0 MEM1") as "%LOAD". des. rewrite LOAD. rred. *)
+  (*   iApply stsim_tauR. rred. *)
+  (*   rewrite close_itree_call. rred. *)
+  (*   iApply lock_yourturn_yieldR. eapply NEQ. *)
+  (*   iSplitL "MYTK TKS MEM0 MEM1 MEM2 MEM3 ST0 ST1 CASES K". *)
+  (*   iSplitL "MYTK". iFrame. iSplitL "TKS". iFrame. iSplitL "MEM0 MEM1 MEM2 MEM3". iFrame. *)
+  (*   iSplitL "ST0 ST1". iFrame. iSplitL "CASES". iFrame. iFrame. *)
+  (*   iIntros "[MYTK RIGHT]". rred. *)
+  (*   rename now into now_old. clear mem own l tks next myt LOAD LOAD0. *)
 
-    iopen 0 "I" "K". do 7 iDestruct "I" as "[% I]". iDestruct "I" as "[TKS [MEM [ST CASES]]]".
-    destruct (Nat.eq_dec mytk now); subst.
-    { iClear "CIH". iApply lock_myturn2. auto.
-      iSplitL "MYTK". iFrame. iSplitL "MYN". iFrame. iSplitL "TKS". iFrame.
-      iSplitL "MEM". iFrame. iSplitL "ST". iFrame. iSplitL "CASES". iFrame.
-      iFrame.
-    }
+  (*   iopen 0 "I" "K". do 7 iDestruct "I" as "[% I]". iDestruct "I" as "[TKS [MEM [ST CASES]]]". *)
+  (*   destruct (Nat.eq_dec mytk now); subst. *)
+  (*   { iClear "CIH". iApply lock_myturn2. auto. *)
+  (*     iSplitL "MYTK". iFrame. iSplitL "MYN". iFrame. iSplitL "TKS". iFrame. *)
+  (*     iSplitL "MEM". iFrame. iSplitL "ST". iFrame. iSplitL "CASES". iFrame. *)
+  (*     iFrame. *)
+  (*   } *)
 
-    iPoseProof (mytk_find_some with "[MYTK TKS]") as "%FIND". iFrame.
-    rename n into NEQ2. iPoseProof (yourturn_range with "CASES") as "%LT". eapply FIND. auto.
-    clear NEQ2. iDestruct "CASES" as "[[%CT I] | [%CF [I | [I | I]]]]".
-    { subst own. iApply lock_yourturn_coind. auto. iSplit. iApply "CIH".
-      iSplitL "MYN". iFrame. iSplitL "MYTK". iFrame. iSplitL "TKS". iFrame.
-      iSplitL "MEM". iFrame. iSplitL "ST". iFrame. iSplitL "I". iFrame. iFrame.
-    }
+  (*   iPoseProof (mytk_find_some with "[MYTK TKS]") as "%FIND". iFrame. *)
+  (*   rename n into NEQ2. iPoseProof (yourturn_range with "CASES") as "%LT". eapply FIND. auto. *)
+  (*   clear NEQ2. iDestruct "CASES" as "[[%CT I] | [%CF [I | [I | I]]]]". *)
+  (*   { subst own. iApply lock_yourturn_coind. auto. iSplit. iApply "CIH". *)
+  (*     iSplitL "MYN". iFrame. iSplitL "MYTK". iFrame. iSplitL "TKS". iFrame. *)
+  (*     iSplitL "MEM". iFrame. iSplitL "ST". iFrame. iSplitL "I". iFrame. iFrame. *)
+  (*   } *)
 
-    { iPoseProof (ticket_lock_inv_mem_mono with "MEM") as "#MONOTK2".
-      iAssert (⌜now_past <= now⌝)%I with "[MEM]" as "%PROG".
-      { iDestruct "MEM" as "[MEM0 [MEM1 [MEM2 [MEM3 MEM4]]]]".
-        iPoseProof (black_white_compare with "MONOTK MEM4") as "%". auto.
-      }
-      iApply lock_yourturn_ind0. apply LT.
-      { clear IHo. move LT before IH. move PROG before LT. clear_upto PROG.
-        intros y H. eapply IH. lia.
-      }
-      auto.
-      iSplit.
-      { iClear "MYN MYTK RIGHT TKS MEM ST I K". iModIntro. iSplit. iApply "CIH". auto. }
-      iSplitL "MYN". iFrame. iSplitL "MYTK". iFrame. iSplitL "TKS". iFrame. iSplitL "MEM". iFrame.
-      iSplitL "ST". subst. iFrame. iSplitR "K". 2: iFrame.
-      iFrame.
-    }
+  (*   { iPoseProof (ticket_lock_inv_mem_mono with "MEM") as "#MONOTK2". *)
+  (*     iAssert (⌜now_past <= now⌝)%I with "[MEM]" as "%PROG". *)
+  (*     { iDestruct "MEM" as "[MEM0 [MEM1 [MEM2 [MEM3 MEM4]]]]". *)
+  (*       iPoseProof (black_white_compare with "MONOTK MEM4") as "%". auto. *)
+  (*     } *)
+  (*     iApply lock_yourturn_ind0. apply LT. *)
+  (*     { clear IHo. move LT before IH. move PROG before LT. clear_upto PROG. *)
+  (*       intros y H. eapply IH. lia. *)
+  (*     } *)
+  (*     auto. *)
+  (*     iSplit. *)
+  (*     { iClear "MYN MYTK RIGHT TKS MEM ST I K". iModIntro. iSplit. iApply "CIH". auto. } *)
+  (*     iSplitL "MYN". iFrame. iSplitL "MYTK". iFrame. iSplitL "TKS". iFrame. iSplitL "MEM". iFrame. *)
+  (*     iSplitL "ST". subst. iFrame. iSplitR "K". 2: iFrame. *)
+  (*     iFrame. *)
+  (*   } *)
 
-    { iPoseProof (unlocked0_contra with "I") as "%FF". eauto. inv FF. }
+  (*   { iPoseProof (unlocked0_contra with "I") as "%FF". eauto. inv FF. } *)
 
-    { iPoseProof (ticket_lock_inv_mem_mono with "MEM") as "#MONOTK2".
-      do 2 iDestruct "I" as "[% I]". iDestruct "I" as "[I0 [%I1 [%I2 [I3 [I4 I5]]]]]".
-      do 3 iDestruct "I5" as "[% I5]". iDestruct "I5" as "[I5 [I6 [I7 [I8 [I9 I10]]]]]".
-      iPoseProof (black_white_compare with "MONOW I5") as "%LE".
-      inv LE.
-      { remember (mytk - now) as ind. specialize (IH ind).
-        iApply IH.
-        { subst ind. lia. }
-        { auto. }
-        { eapply LT. }
-        { eapply Heqind. }
-        iSplit.
-        { iClear "MYN MYTK RIGHT TKS MEM ST I0 I3 I4 I5 I6 I7 I8 I9 I10 K".
-          iModIntro. iSplit. iApply "CIH". auto.
-        }
-        iSplitL "MYN". iFrame. iSplitL "MYTK". iFrame. iSplitL "TKS". iFrame.
-        iSplitL "ST". iFrame. iSplitR "K MEM". 2: iFrame.
-        iRight. iSplit. auto. iRight. iRight. iFrame. iExists yourt, waits.
-        iSplit. auto. iSplit. auto. iFrame. iExists k, o, u. iFrame.
-      }
-      { inv ORD. hexploit H0. lia. i. clear H H0. subst k.
-        iClear "MONOTK2".
-        iPoseProof (ObligationRA.duty_correl_thread with "I8") as "#COR".
-        { ss. left; eauto. }
-        iPoseProof (ObligationRA.correl_thread_correlate with "COR RIGHT") as ">[DROP | FF]".
-        2:{ iPoseProof (ObligationRA.pending_not_shot with "I7 FF") as "%FF". inv FF. }
-        iPoseProof (ObligationRA.black_white_decr with "BLK DROP") as ">[%o_now [#OBLK2 %DROP]]".
-        iClear "BLK".
-        specialize (IHo o_now). iApply IHo.
-        { rewrite Hessenberg.add_S_r in DROP. rewrite Hessenberg.add_O_r in DROP.
-          eapply Ord.lt_le_lt. 2: eapply DROP. apply Ord.S_lt.
-        }
-        { auto. }
-        iSplit.
-        { iClear "MYN MYTK TKS MEM ST I0 I3 I4 I5 I6 I7 I8 I9 I10 K".
-          iModIntro. iSplit. iApply "CIH". auto.
-        }
-        iSplitL "MYN". iFrame. iSplitL "MYTK". iFrame. iSplitL "TKS". iFrame.
-        iSplitL "MEM". iFrame. iSplitL "ST". iFrame. iSplitR "K". 2: iFrame.
-        iFrame. iExists yourt, waits.
-        iSplit. auto. iSplit. auto. iFrame. iExists _, _, u. iFrame.
-      }
-    }
-  Qed.
+  (*   { iPoseProof (ticket_lock_inv_mem_mono with "MEM") as "#MONOTK2". *)
+  (*     do 2 iDestruct "I" as "[% I]". iDestruct "I" as "[I0 [%I1 [%I2 [I3 [I4 I5]]]]]". *)
+  (*     do 3 iDestruct "I5" as "[% I5]". iDestruct "I5" as "[I5 [I6 [I7 [I8 [I9 I10]]]]]". *)
+  (*     iPoseProof (black_white_compare with "MONOW I5") as "%LE". *)
+  (*     inv LE. *)
+  (*     { remember (mytk - now) as ind. specialize (IH ind). *)
+  (*       iApply IH. *)
+  (*       { subst ind. lia. } *)
+  (*       { auto. } *)
+  (*       { eapply LT. } *)
+  (*       { eapply Heqind. } *)
+  (*       iSplit. *)
+  (*       { iClear "MYN MYTK RIGHT TKS MEM ST I0 I3 I4 I5 I6 I7 I8 I9 I10 K". *)
+  (*         iModIntro. iSplit. iApply "CIH". auto. *)
+  (*       } *)
+  (*       iSplitL "MYN". iFrame. iSplitL "MYTK". iFrame. iSplitL "TKS". iFrame. *)
+  (*       iSplitL "ST". iFrame. iSplitR "K MEM". 2: iFrame. *)
+  (*       iRight. iSplit. auto. iRight. iRight. iFrame. iExists yourt, waits. *)
+  (*       iSplit. auto. iSplit. auto. iFrame. iExists k, o, u. iFrame. *)
+  (*     } *)
+  (*     { inv ORD. hexploit H0. lia. i. clear H H0. subst k. *)
+  (*       iClear "MONOTK2". *)
+  (*       iPoseProof (ObligationRA.duty_correl_thread with "I8") as "#COR". *)
+  (*       { ss. left; eauto. } *)
+  (*       iPoseProof (ObligationRA.correl_thread_correlate with "COR RIGHT") as ">[DROP | FF]". *)
+  (*       2:{ iPoseProof (ObligationRA.pending_not_shot with "I7 FF") as "%FF". inv FF. } *)
+  (*       iPoseProof (ObligationRA.black_white_decr with "BLK DROP") as ">[%o_now [#OBLK2 %DROP]]". *)
+  (*       iClear "BLK". *)
+  (*       specialize (IHo o_now). iApply IHo. *)
+  (*       { rewrite Hessenberg.add_S_r in DROP. rewrite Hessenberg.add_O_r in DROP. *)
+  (*         eapply Ord.lt_le_lt. 2: eapply DROP. apply Ord.S_lt. *)
+  (*       } *)
+  (*       { auto. } *)
+  (*       iSplit. *)
+  (*       { iClear "MYN MYTK TKS MEM ST I0 I3 I4 I5 I6 I7 I8 I9 I10 K". *)
+  (*         iModIntro. iSplit. iApply "CIH". auto. *)
+  (*       } *)
+  (*       iSplitL "MYN". iFrame. iSplitL "MYTK". iFrame. iSplitL "TKS". iFrame. *)
+  (*       iSplitL "MEM". iFrame. iSplitL "ST". iFrame. iSplitR "K". 2: iFrame. *)
+  (*       iFrame. iExists yourt, waits. *)
+  (*       iSplit. auto. iSplit. auto. iFrame. iExists _, _, u. iFrame. *)
+  (*     } *)
+  (*   } *)
+  (* Qed. *)
 
-  Lemma correct_lock tid:
+  Lemma correct_lock tid tvw:
     ((own_thread tid)
        ∗ (ObligationRA.duty (inl tid) [])
     )
@@ -2134,9 +2193,9 @@ Section SIM.
       (stsim I tid (topset I) ibot7 ibot7
              (fun r_src r_tgt => own_thread tid ** ObligationRA.duty (inl tid) [] ** ⌜r_src = r_tgt⌝)
              false false
-             (AbsLock.lock_fun tt)
-             (OMod.close_itree TicketLock.omod (WMem.mod TicketLock.gvs)
-                               (TicketLock.lock_fun tt))).
+             (AbsLockW.lock_fun tvw)
+             (OMod.close_itree TicketLockW.omod (WMem.mod)
+                               (TicketLockW.lock_fun tvw))).
   Proof.
     iIntros "[MYTH DUTY]".
     iApply lock_enqueue. iSplitL. iFrame.
